<?xml version="1.0"?>
<rdf:RDF xmlns="https://w3id.org/cerif2/"
     xml:base="https://w3id.org/cerif2/"
     xmlns:owl="http://www.w3.org/2002/07/owl#"
     xmlns:rdf="http://www.w3.org/1999/02/22-rdf-syntax-ns#"
     xmlns:xml="http://www.w3.org/XML/1998/namespace"
     xmlns:xsd="http://www.w3.org/2001/XMLSchema#"
     xmlns:rdfs="http://www.w3.org/2000/01/rdf-schema#">
    <owl:Ontology rdf:about="https://w3id.org/cerif2/"/>
    


    <!-- 
    ///////////////////////////////////////////////////////////////////////////////////////
    //
    // Datatypes
    //
    ///////////////////////////////////////////////////////////////////////////////////////
     -->


    


    <!-- http://www.w3.org/2001/XMLSchema#date -->


    <rdfs:Datatype rdf:about="http://www.w3.org/2001/XMLSchema#date"/>
    


    <!-- http://www.w3.org/2001/XMLSchema#gYear -->


    <rdfs:Datatype rdf:about="http://www.w3.org/2001/XMLSchema#gYear"/>
    


    <!-- http://www.w3.org/2001/XMLSchema#gYearMonth -->


    <rdfs:Datatype rdf:about="http://www.w3.org/2001/XMLSchema#gYearMonth"/>
    


    <!-- https://w3id.org/cerif2/Boolean -->


    <rdfs:Datatype rdf:about="https://w3id.org/cerif2/Boolean"/>
    


    <!-- https://w3id.org/cerif2/DOI_ID -->


    <rdfs:Datatype rdf:about="https://w3id.org/cerif2/DOI_ID"/>
    


    <!-- https://w3id.org/cerif2/Date -->


    <rdfs:Datatype rdf:about="https://w3id.org/cerif2/Date">
        <owl:equivalentClass>
            <rdfs:Datatype>
                <owl:unionOf rdf:parseType="Collection">
                    <rdf:Description rdf:about="http://www.w3.org/2001/XMLSchema#date"/>
                    <rdf:Description rdf:about="http://www.w3.org/2001/XMLSchema#gYear"/>
                    <rdf:Description rdf:about="http://www.w3.org/2001/XMLSchema#gYearMonth"/>
                </owl:unionOf>
            </rdfs:Datatype>
        </owl:equivalentClass>
    </rdfs:Datatype>
    


    <!-- https://w3id.org/cerif2/Decimal -->


    <rdfs:Datatype rdf:about="https://w3id.org/cerif2/Decimal"/>
    


    <!-- https://w3id.org/cerif2/FundRef_ID -->


    <rdfs:Datatype rdf:about="https://w3id.org/cerif2/FundRef_ID"/>
    


    <!-- https://w3id.org/cerif2/ISNI_ID -->


    <rdfs:Datatype rdf:about="https://w3id.org/cerif2/ISNI_ID"/>
    


    <!-- https://w3id.org/cerif2/ISO_15924_Alpha4_Code -->


    <rdfs:Datatype rdf:about="https://w3id.org/cerif2/ISO_15924_Alpha4_Code"/>
    


    <!-- https://w3id.org/cerif2/ISO_3166_Alpha2_Code -->


    <rdfs:Datatype rdf:about="https://w3id.org/cerif2/ISO_3166_Alpha2_Code"/>
    


    <!-- https://w3id.org/cerif2/ISO_4217_Alpha_Code -->


    <rdfs:Datatype rdf:about="https://w3id.org/cerif2/ISO_4217_Alpha_Code"/>
    


    <!-- https://w3id.org/cerif2/ISO_639_1_Alpha2_Code -->


    <rdfs:Datatype rdf:about="https://w3id.org/cerif2/ISO_639_1_Alpha2_Code"/>
    


    <!-- https://w3id.org/cerif2/ISO_639_2B_Alpha3_Code -->


    <rdfs:Datatype rdf:about="https://w3id.org/cerif2/ISO_639_2B_Alpha3_Code"/>
    


    <!-- https://w3id.org/cerif2/ISO_639_2T_Alpha3_Code -->


    <rdfs:Datatype rdf:about="https://w3id.org/cerif2/ISO_639_2T_Alpha3_Code"/>
    


    <!-- https://w3id.org/cerif2/Local_Agent_ID -->


    <rdfs:Datatype rdf:about="https://w3id.org/cerif2/Local_Agent_ID"/>
    


    <!-- https://w3id.org/cerif2/Local_Resource_ID -->


    <rdfs:Datatype rdf:about="https://w3id.org/cerif2/Local_Resource_ID"/>
    


    <!-- https://w3id.org/cerif2/Multilingual_String -->


    <rdfs:Datatype rdf:about="https://w3id.org/cerif2/Multilingual_String"/>
    


    <!-- https://w3id.org/cerif2/ORCID_iD -->


    <rdfs:Datatype rdf:about="https://w3id.org/cerif2/ORCID_iD"/>
    


    <!-- https://w3id.org/cerif2/ROR_ID -->


    <rdfs:Datatype rdf:about="https://w3id.org/cerif2/ROR_ID"/>
    


    <!-- https://w3id.org/cerif2/String -->


    <rdfs:Datatype rdf:about="https://w3id.org/cerif2/String"/>
    


    <!-- https://w3id.org/cerif2/Time -->


    <rdfs:Datatype rdf:about="https://w3id.org/cerif2/Time"/>
    


    <!-- https://w3id.org/cerif2/URI -->


    <rdfs:Datatype rdf:about="https://w3id.org/cerif2/URI"/>
    


    <!-- https://w3id.org/cerif2/Website_Address -->


    <rdfs:Datatype rdf:about="https://w3id.org/cerif2/Website_Address"/>
    


    <!-- https://w3id.org/cerif2/Wikidata_ID -->


    <rdfs:Datatype rdf:about="https://w3id.org/cerif2/Wikidata_ID"/>
    


    <!-- 
    ///////////////////////////////////////////////////////////////////////////////////////
    //
    // Object Properties
    //
    ///////////////////////////////////////////////////////////////////////////////////////
     -->


    


    <!-- https://w3id.org/cerif2/Acknowledgement_Statement#testify -->


    <owl:ObjectProperty rdf:about="https://w3id.org/cerif2/Acknowledgement_Statement#testify">
        <owl:inverseOf rdf:resource="https://w3id.org/cerif2/Contribution#isTestifiedBy"/>
        <rdfs:domain rdf:resource="https://w3id.org/cerif2/Acknowledgement_Statement"/>
        <rdfs:range rdf:resource="https://w3id.org/cerif2/Contribution"/>
        <rdfs:comment xml:lang="en">An Acknowledgement Statement testifies a [Contribution](../entities/Contribution.md).</rdfs:comment>
    </owl:ObjectProperty>
    


    <!-- https://w3id.org/cerif2/Activity#dateRange -->


    <owl:ObjectProperty rdf:about="https://w3id.org/cerif2/Activity#dateRange">
        <rdfs:domain rdf:resource="https://w3id.org/cerif2/Activity"/>
        <rdfs:range rdf:resource="https://w3id.org/cerif2/Date_Range"/>
    </owl:ObjectProperty>
    


    <!-- https://w3id.org/cerif2/Activity#hasActor -->


    <owl:ObjectProperty rdf:about="https://w3id.org/cerif2/Activity#hasActor">
        <owl:inverseOf rdf:resource="https://w3id.org/cerif2/Agent#isActorIn"/>
        <rdfs:domain rdf:resource="https://w3id.org/cerif2/Activity"/>
        <rdfs:range rdf:resource="https://w3id.org/cerif2/Agent"/>
        <rdfs:comment xml:lang="en">An Activity typically has the actor: an instance of [Agent](../entities/Agent.md). For some subclasses of Activity, the Agent may not be known or disclosed (e.g. for blind reviews). Also if the actor uses a pseudonym, their identity (and sometimes event the type) are unknown, in which case just a display name is available.</rdfs:comment>
    </owl:ObjectProperty>
    


    <!-- https://w3id.org/cerif2/Activity#hasAffiliationStatement -->


    <owl:ObjectProperty rdf:about="https://w3id.org/cerif2/Activity#hasAffiliationStatement">
        <owl:inverseOf rdf:resource="https://w3id.org/cerif2/Affiliation_Statement#isUsedIn"/>
        <rdfs:domain rdf:resource="https://w3id.org/cerif2/Activity"/>
        <rdfs:range rdf:resource="https://w3id.org/cerif2/Affiliation_Statement"/>
        <rdfs:comment xml:lang="en">An Activity can have any number of [Affiliation Statements](../entities/Affiliation_Statement.md).</rdfs:comment>
    </owl:ObjectProperty>
    


    <!-- https://w3id.org/cerif2/Activity#isCoveredBy -->


    <owl:ObjectProperty rdf:about="https://w3id.org/cerif2/Activity#isCoveredBy">
        <owl:inverseOf rdf:resource="https://w3id.org/cerif2/Funding#covers"/>
        <rdfs:domain rdf:resource="https://w3id.org/cerif2/Activity"/>
        <rdfs:range rdf:resource="https://w3id.org/cerif2/Funding"/>
        <rdfs:comment xml:lang="en">An Activity can be covered by any number of [Fundings](../entities/Funding.md).</rdfs:comment>
    </owl:ObjectProperty>
    


    <!-- https://w3id.org/cerif2/Activity#isEvidencedBy -->


    <owl:ObjectProperty rdf:about="https://w3id.org/cerif2/Activity#isEvidencedBy">
        <owl:inverseOf rdf:resource="https://w3id.org/cerif2/Document#proves"/>
        <rdfs:domain rdf:resource="https://w3id.org/cerif2/Activity"/>
        <rdfs:range rdf:resource="https://w3id.org/cerif2/Document"/>
        <rdfs:comment xml:lang="en">An Activity can be evidenced by any number of [Documents](../entities/Document.md).</rdfs:comment>
    </owl:ObjectProperty>
    


    <!-- https://w3id.org/cerif2/Affiliation_Statement#hasInstitution -->


    <owl:ObjectProperty rdf:about="https://w3id.org/cerif2/Affiliation_Statement#hasInstitution">
        <owl:inverseOf rdf:resource="https://w3id.org/cerif2/Organisation_Unit#isTheInstitutionIn"/>
        <rdfs:domain rdf:resource="https://w3id.org/cerif2/Affiliation_Statement"/>
        <rdfs:range rdf:resource="https://w3id.org/cerif2/Organisation_Unit"/>
        <rdfs:comment xml:lang="en">An Affiliation Statement has institution, an instance of [Organisation Units](../entities/Organisation_Unit.md).</rdfs:comment>
    </owl:ObjectProperty>
    


    <!-- https://w3id.org/cerif2/Affiliation_Statement#hasOrganisationUnit -->


    <owl:ObjectProperty rdf:about="https://w3id.org/cerif2/Affiliation_Statement#hasOrganisationUnit">
        <owl:inverseOf rdf:resource="https://w3id.org/cerif2/Organisation_Unit#isTheOrganisationUnitIn"/>
        <rdfs:domain rdf:resource="https://w3id.org/cerif2/Affiliation_Statement"/>
        <rdfs:range rdf:resource="https://w3id.org/cerif2/Organisation_Unit"/>
        <rdfs:comment xml:lang="en">An Affiliation Statement can optionally have an organisation unit, an instance of [Organisation Unit](../entities/Organisation_Unit.md).</rdfs:comment>
    </owl:ObjectProperty>
    


    <!-- https://w3id.org/cerif2/Affiliation_Statement#hasPerson -->


    <owl:ObjectProperty rdf:about="https://w3id.org/cerif2/Affiliation_Statement#hasPerson">
        <owl:inverseOf rdf:resource="https://w3id.org/cerif2/Person#isThePersonIn"/>
        <rdfs:domain rdf:resource="https://w3id.org/cerif2/Affiliation_Statement"/>
        <rdfs:range rdf:resource="https://w3id.org/cerif2/Person"/>
        <rdfs:comment xml:lang="en">An Affiliation Statement typically has the person, an instance of [Person](../entities/Person.md).</rdfs:comment>
    </owl:ObjectProperty>
    


    <!-- https://w3id.org/cerif2/Affiliation_Statement#isTheResultOf -->


    <owl:ObjectProperty rdf:about="https://w3id.org/cerif2/Affiliation_Statement#isTheResultOf">
        <owl:inverseOf rdf:resource="https://w3id.org/cerif2/Involvement#isTheFoundationFor"/>
        <rdfs:domain rdf:resource="https://w3id.org/cerif2/Affiliation_Statement"/>
        <rdfs:range rdf:resource="https://w3id.org/cerif2/Involvement"/>
        <rdfs:comment xml:lang="en">An Affiliation Statement might be a result of an Agent [Involvement](../entities/Involvement.md).</rdfs:comment>
    </owl:ObjectProperty>
    


    <!-- https://w3id.org/cerif2/Affiliation_Statement#isUsedIn -->


    <owl:ObjectProperty rdf:about="https://w3id.org/cerif2/Affiliation_Statement#isUsedIn">
        <rdfs:domain rdf:resource="https://w3id.org/cerif2/Affiliation_Statement"/>
        <rdfs:range rdf:resource="https://w3id.org/cerif2/Activity"/>
        <rdfs:comment xml:lang="en">An Affiliation Statement can be used in any number of [Activities](../entities/Activity.md).</rdfs:comment>
    </owl:ObjectProperty>
    


    <!-- https://w3id.org/cerif2/Affiliation_Statement#position -->


    <owl:ObjectProperty rdf:about="https://w3id.org/cerif2/Affiliation_Statement#position">
        <rdfs:domain rdf:resource="https://w3id.org/cerif2/Affiliation_Statement"/>
        <rdfs:range rdf:resource="https://w3id.org/cerif2/Position"/>
    </owl:ObjectProperty>
    


    <!-- https://w3id.org/cerif2/Agent#awardsPrize -->


    <owl:ObjectProperty rdf:about="https://w3id.org/cerif2/Agent#awardsPrize">
        <rdfs:domain rdf:resource="https://w3id.org/cerif2/Agent"/>
        <rdfs:range rdf:resource="https://w3id.org/cerif2/Event"/>
        <rdfs:comment xml:lang="en">An Agent can award any number of [Prize Awards](../entities/Prize_Award.md).</rdfs:comment>
    </owl:ObjectProperty>
    


    <!-- https://w3id.org/cerif2/Agent#hasIdentifier -->


    <owl:ObjectProperty rdf:about="https://w3id.org/cerif2/Agent#hasIdentifier">
        <owl:inverseOf rdf:resource="https://w3id.org/cerif2/Agent_Identifier#isAssignedTo"/>
        <rdfs:domain rdf:resource="https://w3id.org/cerif2/Agent"/>
        <rdfs:range rdf:resource="https://w3id.org/cerif2/Agent_Identifier"/>
        <rdfs:comment xml:lang="en">An Agent can be assigned any number of [Agent Identifiers](../entities/Agent_Identifier.md).</rdfs:comment>
    </owl:ObjectProperty>
    


    <!-- https://w3id.org/cerif2/Agent#isActorIn -->


    <owl:ObjectProperty rdf:about="https://w3id.org/cerif2/Agent#isActorIn">
        <rdfs:domain rdf:resource="https://w3id.org/cerif2/Agent"/>
        <rdfs:range rdf:resource="https://w3id.org/cerif2/Activity"/>
        <rdfs:comment xml:lang="en">An Agent can be the actor in any number of [Activities](../entities/Activity.md).</rdfs:comment>
    </owl:ObjectProperty>
    


    <!-- https://w3id.org/cerif2/Agent#isAddresseeOf -->


    <owl:ObjectProperty rdf:about="https://w3id.org/cerif2/Agent#isAddresseeOf">
        <owl:inverseOf rdf:resource="https://w3id.org/cerif2/Resource_Request#hasAddressee"/>
        <rdfs:domain rdf:resource="https://w3id.org/cerif2/Agent"/>
        <rdfs:range rdf:resource="https://w3id.org/cerif2/Resource_Request"/>
        <rdfs:comment xml:lang="en">An Agent can be the addressee of any number of [Resource Request](../entities/Resource_Request.md).</rdfs:comment>
    </owl:ObjectProperty>
    


    <!-- https://w3id.org/cerif2/Agent#isAgentIn1 -->


    <owl:ObjectProperty rdf:about="https://w3id.org/cerif2/Agent#isAgentIn1">
        <owl:inverseOf rdf:resource="https://w3id.org/cerif2/Expertise_and_Skills_Possession#byAgent"/>
        <rdfs:domain rdf:resource="https://w3id.org/cerif2/Agent"/>
        <rdfs:range rdf:resource="https://w3id.org/cerif2/Expertise_and_Skills_Possession"/>
        <rdfs:comment xml:lang="en">An Agent can be the agent in any number of [Expertise and Skills Possessions](../entities/Expertise_and_Skills_Possession.md).</rdfs:comment>
    </owl:ObjectProperty>
    


    <!-- https://w3id.org/cerif2/Agent#isAgentIn2 -->


    <owl:ObjectProperty rdf:about="https://w3id.org/cerif2/Agent#isAgentIn2">
        <owl:inverseOf rdf:resource="https://w3id.org/cerif2/Expertise_and_Time_and_Effort#byAgent"/>
        <rdfs:domain rdf:resource="https://w3id.org/cerif2/Agent"/>
        <rdfs:range rdf:resource="https://w3id.org/cerif2/Expertise_and_Time_and_Effort"/>
        <rdfs:comment xml:lang="en">An Agent can be the agent in any number of [Expertise and Time and Effort](../entities/Expertise_and_Time_and_Effort.md) instances.</rdfs:comment>
    </owl:ObjectProperty>
    


    <!-- https://w3id.org/cerif2/Agent#isRecipientOf -->


    <owl:ObjectProperty rdf:about="https://w3id.org/cerif2/Agent#isRecipientOf">
        <owl:inverseOf rdf:resource="https://w3id.org/cerif2/Prize_Award#hasRecipient"/>
        <rdfs:domain rdf:resource="https://w3id.org/cerif2/Agent"/>
        <rdfs:range rdf:resource="https://w3id.org/cerif2/Prize_Award"/>
        <rdfs:comment xml:lang="en">An Agent can be the recipient of any number of [Prize Awards](../entities/Prize_Award.md).</rdfs:comment>
    </owl:ObjectProperty>
    


    <!-- https://w3id.org/cerif2/Agent#isRequesterIn -->


    <owl:ObjectProperty rdf:about="https://w3id.org/cerif2/Agent#isRequesterIn">
        <owl:inverseOf rdf:resource="https://w3id.org/cerif2/Resource_Request#hasRequester"/>
        <rdfs:domain rdf:resource="https://w3id.org/cerif2/Agent"/>
        <rdfs:range rdf:resource="https://w3id.org/cerif2/Resource_Request"/>
        <rdfs:comment xml:lang="en">An Agent can be the requester in any number of [Applications](../entities/Resource_Request.md).</rdfs:comment>
    </owl:ObjectProperty>
    


    <!-- https://w3id.org/cerif2/Agent#lifetime -->


    <owl:ObjectProperty rdf:about="https://w3id.org/cerif2/Agent#lifetime">
        <rdfs:domain rdf:resource="https://w3id.org/cerif2/Agent"/>
        <rdfs:range rdf:resource="https://w3id.org/cerif2/Date_Range"/>
    </owl:ObjectProperty>
    


    <!-- https://w3id.org/cerif2/Agent#made -->


    <owl:ObjectProperty rdf:about="https://w3id.org/cerif2/Agent#made">
        <owl:inverseOf rdf:resource="https://w3id.org/cerif2/Decision#madeBy"/>
        <rdfs:domain rdf:resource="https://w3id.org/cerif2/Agent"/>
        <rdfs:range rdf:resource="https://w3id.org/cerif2/Decision"/>
        <rdfs:comment xml:lang="en">An Agent can make a [Decision](../entities/Decision.md) on Resource Request based or not on Evaluation Outcomes.</rdfs:comment>
    </owl:ObjectProperty>
    


    <!-- https://w3id.org/cerif2/Agent#solicits -->


    <owl:ObjectProperty rdf:about="https://w3id.org/cerif2/Agent#solicits">
        <owl:inverseOf rdf:resource="https://w3id.org/cerif2/Resource_Offer#isSolicitedBy"/>
        <rdfs:domain rdf:resource="https://w3id.org/cerif2/Agent"/>
        <rdfs:range rdf:resource="https://w3id.org/cerif2/Resource_Offer"/>
        <rdfs:comment xml:lang="en">An Agent can solicit any number of [Resource Offers](../entities/Resource_Offer.md).</rdfs:comment>
    </owl:ObjectProperty>
    


    <!-- https://w3id.org/cerif2/Agent_Identifier#isAssignedTo -->


    <owl:ObjectProperty rdf:about="https://w3id.org/cerif2/Agent_Identifier#isAssignedTo">
        <rdfs:domain rdf:resource="https://w3id.org/cerif2/Agent_Identifier"/>
        <rdfs:range rdf:resource="https://w3id.org/cerif2/Agent"/>
        <rdfs:comment xml:lang="en">An Agent Identifier is assigned to an [Agent](../entities/Agent.md).</rdfs:comment>
    </owl:ObjectProperty>
    


    <!-- https://w3id.org/cerif2/Application#inResponseTo -->


    <owl:ObjectProperty rdf:about="https://w3id.org/cerif2/Application#inResponseTo">
        <owl:inverseOf rdf:resource="https://w3id.org/cerif2/Call_for_Applications#hasApplication"/>
        <rdfs:domain rdf:resource="https://w3id.org/cerif2/Application"/>
        <rdfs:range rdf:resource="https://w3id.org/cerif2/Call_for_Applications"/>
        <rdfs:comment xml:lang="en">An Application can optionally reference the [Call for Applications](../entities/Call_for_Applications.md) it responds to.</rdfs:comment>
    </owl:ObjectProperty>
    


    <!-- https://w3id.org/cerif2/Call_for_Applications#hasApplication -->


    <owl:ObjectProperty rdf:about="https://w3id.org/cerif2/Call_for_Applications#hasApplication">
        <rdfs:domain rdf:resource="https://w3id.org/cerif2/Call_for_Applications"/>
        <rdfs:range rdf:resource="https://w3id.org/cerif2/Application"/>
        <rdfs:comment xml:lang="en">A Call for Applications can reference the [Applications](../entities/Application.md) that make a reference to it.</rdfs:comment>
    </owl:ObjectProperty>
    


    <!-- https://w3id.org/cerif2/Condition#appliesTo -->


    <owl:ObjectProperty rdf:about="https://w3id.org/cerif2/Condition#appliesTo">
        <owl:inverseOf rdf:resource="https://w3id.org/cerif2/Resource_Offer#hasCondition"/>
        <rdfs:domain rdf:resource="https://w3id.org/cerif2/Condition"/>
        <rdfs:range rdf:resource="https://w3id.org/cerif2/Resource_Offer"/>
        <rdfs:comment xml:lang="en">A Condition applies to a [Resource Offer](../entities/Resource_Offer.md).</rdfs:comment>
    </owl:ObjectProperty>
    


    <!-- https://w3id.org/cerif2/Contribution#hasContributionStatement -->


    <owl:ObjectProperty rdf:about="https://w3id.org/cerif2/Contribution#hasContributionStatement">
        <owl:inverseOf rdf:resource="https://w3id.org/cerif2/Contribution_Statement#references"/>
        <rdfs:domain rdf:resource="https://w3id.org/cerif2/Contribution"/>
        <rdfs:range rdf:resource="https://w3id.org/cerif2/Contribution_Statement"/>
        <rdfs:comment xml:lang="en">A Contribution can have any number of [Contribution Statements](../entities/Contribution_Statement.md).</rdfs:comment>
    </owl:ObjectProperty>
    


    <!-- https://w3id.org/cerif2/Contribution#isTestifiedBy -->


    <owl:ObjectProperty rdf:about="https://w3id.org/cerif2/Contribution#isTestifiedBy">
        <rdfs:domain rdf:resource="https://w3id.org/cerif2/Contribution"/>
        <rdfs:range rdf:resource="https://w3id.org/cerif2/Acknowledgement_Statement"/>
        <rdfs:comment xml:lang="en">A Contribution can be testified by any number of [Acknowledgement Statements](../entities/Acknowledgement_Statement.md).</rdfs:comment>
    </owl:ObjectProperty>
    


    <!-- https://w3id.org/cerif2/Contribution_Statement#isDetailedIn -->


    <owl:ObjectProperty rdf:about="https://w3id.org/cerif2/Contribution_Statement#isDetailedIn">
        <owl:inverseOf rdf:resource="https://w3id.org/cerif2/Resource_Usage_Statement#details"/>
        <rdfs:domain rdf:resource="https://w3id.org/cerif2/Contribution_Statement"/>
        <rdfs:range rdf:resource="https://w3id.org/cerif2/Resource_Usage_Statement"/>
        <rdfs:comment xml:lang="en">A Contribution Statement can be detailed in any number of [Resource Usage Statements](../entities/Resource_Usage_Statement.md).</rdfs:comment>
    </owl:ObjectProperty>
    


    <!-- https://w3id.org/cerif2/Contribution_Statement#provides -->


    <owl:ObjectProperty rdf:about="https://w3id.org/cerif2/Contribution_Statement#provides">
        <owl:inverseOf rdf:resource="https://w3id.org/cerif2/Resource#isProvidedBy"/>
        <rdfs:domain rdf:resource="https://w3id.org/cerif2/Contribution_Statement"/>
        <rdfs:range rdf:resource="https://w3id.org/cerif2/Resource"/>
        <rdfs:comment xml:lang="en">A Contribution Statement can optionally provide any number of [Resources](../entities/Resource.md). These resources can be funding, expertise, equipment, time or space.</rdfs:comment>
    </owl:ObjectProperty>
    


    <!-- https://w3id.org/cerif2/Contribution_Statement#references -->


    <owl:ObjectProperty rdf:about="https://w3id.org/cerif2/Contribution_Statement#references">
        <rdfs:domain rdf:resource="https://w3id.org/cerif2/Contribution_Statement"/>
        <rdfs:range rdf:resource="https://w3id.org/cerif2/Contribution"/>
        <rdfs:comment xml:lang="en">A Contribution Statement references the [Contribution](../entities/Contribution.md) to which it relates.</rdfs:comment>
    </owl:ObjectProperty>
    


    <!-- https://w3id.org/cerif2/Contribution_to_Document#hasTarget -->


    <owl:ObjectProperty rdf:about="https://w3id.org/cerif2/Contribution_to_Document#hasTarget">
        <owl:inverseOf rdf:resource="https://w3id.org/cerif2/Document#hasContribution"/>
        <rdfs:domain rdf:resource="https://w3id.org/cerif2/Contribution_to_Document"/>
        <rdfs:range rdf:resource="https://w3id.org/cerif2/Document"/>
        <rdfs:comment xml:lang="en">A Contribution to Document always references the target [Document](../entities/Document.md).</rdfs:comment>
    </owl:ObjectProperty>
    


    <!-- https://w3id.org/cerif2/Contribution_to_Evaluation_Outcome#hasTarget -->


    <owl:ObjectProperty rdf:about="https://w3id.org/cerif2/Contribution_to_Evaluation_Outcome#hasTarget">
        <owl:inverseOf rdf:resource="https://w3id.org/cerif2/Evaluation_Outcome#hasContribution"/>
        <rdfs:domain rdf:resource="https://w3id.org/cerif2/Contribution_to_Evaluation_Outcome"/>
        <rdfs:range rdf:resource="https://w3id.org/cerif2/Evaluation_Outcome"/>
        <rdfs:comment xml:lang="en">A Contribution to Evaluation Outcome always references the target [Evaluation Outcome](../entities/Evaluation_Outcome.md).</rdfs:comment>
    </owl:ObjectProperty>
    


    <!-- https://w3id.org/cerif2/Contribution_to_Event#hasTarget -->


    <owl:ObjectProperty rdf:about="https://w3id.org/cerif2/Contribution_to_Event#hasTarget">
        <owl:inverseOf rdf:resource="https://w3id.org/cerif2/Event#hasContribution"/>
        <rdfs:domain rdf:resource="https://w3id.org/cerif2/Contribution_to_Event"/>
        <rdfs:range rdf:resource="https://w3id.org/cerif2/Event"/>
        <rdfs:comment xml:lang="en">A Contribution to Event always references the target [Event](../entities/Event.md).</rdfs:comment>
    </owl:ObjectProperty>
    


    <!-- https://w3id.org/cerif2/Contribution_to_Infrastructure#hasTarget -->


    <owl:ObjectProperty rdf:about="https://w3id.org/cerif2/Contribution_to_Infrastructure#hasTarget">
        <owl:inverseOf rdf:resource="https://w3id.org/cerif2/Infrastructure#hasContribution"/>
        <rdfs:domain rdf:resource="https://w3id.org/cerif2/Contribution_to_Infrastructure"/>
        <rdfs:range rdf:resource="https://w3id.org/cerif2/Infrastructure"/>
        <rdfs:comment xml:lang="en">A Contribution to Infrastructure always references the [Infrastructure](../entities/Infrastructure.md) that benefits from it.</rdfs:comment>
    </owl:ObjectProperty>
    


    <!-- https://w3id.org/cerif2/Contribution_to_Prize#hasTarget -->


    <owl:ObjectProperty rdf:about="https://w3id.org/cerif2/Contribution_to_Prize#hasTarget">
        <owl:inverseOf rdf:resource="https://w3id.org/cerif2/Prize#hasContribution"/>
        <rdfs:domain rdf:resource="https://w3id.org/cerif2/Contribution_to_Prize"/>
        <rdfs:range rdf:resource="https://w3id.org/cerif2/Prize"/>
        <rdfs:comment xml:lang="en">A Contribution to Prize always has the target [Prize](../entities/Prize.md).</rdfs:comment>
    </owl:ObjectProperty>
    


    <!-- https://w3id.org/cerif2/Contribution_to_Prize_Award#hasTarget -->


    <owl:ObjectProperty rdf:about="https://w3id.org/cerif2/Contribution_to_Prize_Award#hasTarget">
        <owl:inverseOf rdf:resource="https://w3id.org/cerif2/Prize_Award#hasContribution"/>
        <rdfs:domain rdf:resource="https://w3id.org/cerif2/Contribution_to_Prize_Award"/>
        <rdfs:range rdf:resource="https://w3id.org/cerif2/Prize_Award"/>
        <rdfs:comment xml:lang="en">A Contribution to Prize Award always has the target [Prize Award](../entities/Prize_Award.md).</rdfs:comment>
    </owl:ObjectProperty>
    


    <!-- https://w3id.org/cerif2/Contribution_to_Project#hasTarget -->


    <owl:ObjectProperty rdf:about="https://w3id.org/cerif2/Contribution_to_Project#hasTarget">
        <owl:inverseOf rdf:resource="https://w3id.org/cerif2/Project#hasContribution"/>
        <rdfs:domain rdf:resource="https://w3id.org/cerif2/Contribution_to_Project"/>
        <rdfs:range rdf:resource="https://w3id.org/cerif2/Project"/>
        <rdfs:comment xml:lang="en">A Contribution to Project always references the target [Project](../entities/Project.md).</rdfs:comment>
    </owl:ObjectProperty>
    


    <!-- https://w3id.org/cerif2/Decision#basedOn -->


    <owl:ObjectProperty rdf:about="https://w3id.org/cerif2/Decision#basedOn">
        <owl:inverseOf rdf:resource="https://w3id.org/cerif2/Evaluation_Outcome#providesBasisFor"/>
        <rdfs:domain rdf:resource="https://w3id.org/cerif2/Decision"/>
        <rdfs:range rdf:resource="https://w3id.org/cerif2/Evaluation_Outcome"/>
        <rdfs:comment xml:lang="en">A Decision can be based on any number of [Evaluation Outcomes](../entities/Evaluation_Outcome.md).</rdfs:comment>
    </owl:ObjectProperty>
    


    <!-- https://w3id.org/cerif2/Decision#isADecisionOn -->


    <owl:ObjectProperty rdf:about="https://w3id.org/cerif2/Decision#isADecisionOn">
        <owl:inverseOf rdf:resource="https://w3id.org/cerif2/Resource_Request#hasDecision"/>
        <rdfs:domain rdf:resource="https://w3id.org/cerif2/Decision"/>
        <rdfs:range rdf:resource="https://w3id.org/cerif2/Resource_Request"/>
        <rdfs:comment xml:lang="en">A Resource Request can have a [Decision](../entities/Decision.md) about accepting or refusing request made by addressee.</rdfs:comment>
    </owl:ObjectProperty>
    


    <!-- https://w3id.org/cerif2/Decision#isExpressedIn -->


    <owl:ObjectProperty rdf:about="https://w3id.org/cerif2/Decision#isExpressedIn">
        <owl:inverseOf rdf:resource="https://w3id.org/cerif2/Document#presentsDecision"/>
        <rdfs:domain rdf:resource="https://w3id.org/cerif2/Decision"/>
        <rdfs:range rdf:resource="https://w3id.org/cerif2/Document"/>
        <rdfs:comment xml:lang="en">A Decision can be expressed in a [Document](../entities/Document.md).</rdfs:comment>
    </owl:ObjectProperty>
    


    <!-- https://w3id.org/cerif2/Decision#madeBy -->


    <owl:ObjectProperty rdf:about="https://w3id.org/cerif2/Decision#madeBy">
        <rdfs:domain rdf:resource="https://w3id.org/cerif2/Decision"/>
        <rdfs:range rdf:resource="https://w3id.org/cerif2/Agent"/>
        <rdfs:comment xml:lang="en">A Decision about accepting or refusing request can be made by any number of [Agents](../entities/Agent.md).</rdfs:comment>
    </owl:ObjectProperty>
    


    <!-- https://w3id.org/cerif2/Document#awardedBy -->


    <owl:ObjectProperty rdf:about="https://w3id.org/cerif2/Document#awardedBy">
        <owl:inverseOf rdf:resource="https://w3id.org/cerif2/Prize_Award#awardedForADocument"/>
        <rdfs:domain rdf:resource="https://w3id.org/cerif2/Document"/>
        <rdfs:range rdf:resource="https://w3id.org/cerif2/Prize_Award"/>
        <rdfs:comment xml:lang="en">A Document can be awarded by a [Prize Award](../entities/Prize_Award.md).</rdfs:comment>
    </owl:ObjectProperty>
    


    <!-- https://w3id.org/cerif2/Document#describesResourceOffer -->


    <owl:ObjectProperty rdf:about="https://w3id.org/cerif2/Document#describesResourceOffer">
        <owl:inverseOf rdf:resource="https://w3id.org/cerif2/Resource_Offer#isDescribedBy"/>
        <rdfs:domain rdf:resource="https://w3id.org/cerif2/Document"/>
        <rdfs:range rdf:resource="https://w3id.org/cerif2/Resource_Offer"/>
        <rdfs:comment xml:lang="en">A Document can provide description of a [Resource Offer](../entities/Resource_Offer.md).</rdfs:comment>
    </owl:ObjectProperty>
    


    <!-- https://w3id.org/cerif2/Document#describesResourceRequest -->


    <owl:ObjectProperty rdf:about="https://w3id.org/cerif2/Document#describesResourceRequest">
        <owl:inverseOf rdf:resource="https://w3id.org/cerif2/Resource_Request#isDescribedBy"/>
        <rdfs:domain rdf:resource="https://w3id.org/cerif2/Document"/>
        <rdfs:range rdf:resource="https://w3id.org/cerif2/Resource_Request"/>
        <rdfs:comment xml:lang="en">A Document can provide description of a [Resource Request](../entities/Resource_Request.md).</rdfs:comment>
    </owl:ObjectProperty>
    


    <!-- https://w3id.org/cerif2/Document#hasContribution -->


    <owl:ObjectProperty rdf:about="https://w3id.org/cerif2/Document#hasContribution">
        <rdfs:domain rdf:resource="https://w3id.org/cerif2/Document"/>
        <rdfs:range rdf:resource="https://w3id.org/cerif2/Contribution_to_Document"/>
        <rdfs:comment xml:lang="en">A Document any number of [contributions](../entities/Contribution_to_Document.md) that helped it arise.</rdfs:comment>
    </owl:ObjectProperty>
    


    <!-- https://w3id.org/cerif2/Document#hasPart -->


    <owl:ObjectProperty rdf:about="https://w3id.org/cerif2/Document#hasPart">
        <owl:inverseOf rdf:resource="https://w3id.org/cerif2/Document#isPartOf"/>
        <rdfs:domain rdf:resource="https://w3id.org/cerif2/Document"/>
        <rdfs:range rdf:resource="https://w3id.org/cerif2/Document"/>
        <rdfs:comment xml:lang="en">A Document can have any number of [Documents](../entities/Document.md) as parts. [Contents Location](../datatypes/Contents_Location.md) can be attached to such an association.</rdfs:comment>
    </owl:ObjectProperty>
    


    <!-- https://w3id.org/cerif2/Document#isPartOf -->


    <owl:ObjectProperty rdf:about="https://w3id.org/cerif2/Document#isPartOf">
        <rdfs:domain rdf:resource="https://w3id.org/cerif2/Document"/>
        <rdfs:range rdf:resource="https://w3id.org/cerif2/Document"/>
        <rdfs:comment xml:lang="en">A Document can be part of any number of other [Documents](../entities/Document.md). [Contents Location](../datatypes/Contents_Location.md) can be attached to such an association.</rdfs:comment>
    </owl:ObjectProperty>
    


    <!-- https://w3id.org/cerif2/Document#presentsDecision -->


    <owl:ObjectProperty rdf:about="https://w3id.org/cerif2/Document#presentsDecision">
        <rdfs:domain rdf:resource="https://w3id.org/cerif2/Document"/>
        <rdfs:range rdf:resource="https://w3id.org/cerif2/Decision"/>
        <rdfs:comment xml:lang="en">A Document can present a [Decision](../entities/Decision.md).</rdfs:comment>
    </owl:ObjectProperty>
    


    <!-- https://w3id.org/cerif2/Document#proves -->


    <owl:ObjectProperty rdf:about="https://w3id.org/cerif2/Document#proves">
        <rdfs:domain rdf:resource="https://w3id.org/cerif2/Document"/>
        <rdfs:range rdf:resource="https://w3id.org/cerif2/Activity"/>
        <rdfs:comment xml:lang="en">A Document can provide evidence of any number of [Activities](../entities/Activity.md).</rdfs:comment>
    </owl:ObjectProperty>
    


    <!-- https://w3id.org/cerif2/Document#providesEvidenceOf -->


    <owl:ObjectProperty rdf:about="https://w3id.org/cerif2/Document#providesEvidenceOf">
        <owl:inverseOf rdf:resource="https://w3id.org/cerif2/Expertise_and_Skills_Possession#isEvidencedBy"/>
        <rdfs:domain rdf:resource="https://w3id.org/cerif2/Document"/>
        <rdfs:range rdf:resource="https://w3id.org/cerif2/Expertise_and_Skills_Possession"/>
        <rdfs:comment xml:lang="en">A Document can provide evidence of any number of [Expertise and Skills Possessions](../entities/Expertise_and_Skills_Possession.md).</rdfs:comment>
    </owl:ObjectProperty>
    


    <!-- https://w3id.org/cerif2/Document#publishedAs -->


    <owl:ObjectProperty rdf:about="https://w3id.org/cerif2/Document#publishedAs">
        <owl:inverseOf rdf:resource="https://w3id.org/cerif2/Document_Publication#of"/>
        <rdfs:domain rdf:resource="https://w3id.org/cerif2/Document"/>
        <rdfs:range rdf:resource="https://w3id.org/cerif2/Document_Publication"/>
        <rdfs:comment xml:lang="en">A Document can be published as [Document Publication](../entities/Document_Publication.md), once or even multiple times.</rdfs:comment>
    </owl:ObjectProperty>
    


    <!-- https://w3id.org/cerif2/Document_Publication#in -->


    <owl:ObjectProperty rdf:about="https://w3id.org/cerif2/Document_Publication#in">
        <owl:inverseOf rdf:resource="https://w3id.org/cerif2/Publication_Channel#contains"/>
        <rdfs:domain rdf:resource="https://w3id.org/cerif2/Document_Publication"/>
        <rdfs:range rdf:resource="https://w3id.org/cerif2/Publication_Channel"/>
        <rdfs:comment xml:lang="en">A Document Publication can be published in any number of [Publication Channels](../entities/Publication_Channel.md). [Contents Location](../datatypes/Contents_Location.md) can be attached to such an association.</rdfs:comment>
    </owl:ObjectProperty>
    


    <!-- https://w3id.org/cerif2/Document_Publication#of -->


    <owl:ObjectProperty rdf:about="https://w3id.org/cerif2/Document_Publication#of">
        <rdfs:domain rdf:resource="https://w3id.org/cerif2/Document_Publication"/>
        <rdfs:range rdf:resource="https://w3id.org/cerif2/Document"/>
        <rdfs:comment xml:lang="en">A Document Publication references the published [Document](../entities/Document.md).</rdfs:comment>
    </owl:ObjectProperty>
    


    <!-- https://w3id.org/cerif2/Evaluation_Outcome#hasContribution -->


    <owl:ObjectProperty rdf:about="https://w3id.org/cerif2/Evaluation_Outcome#hasContribution">
        <rdfs:domain rdf:resource="https://w3id.org/cerif2/Evaluation_Outcome"/>
        <rdfs:range rdf:resource="https://w3id.org/cerif2/Contribution_to_Evaluation_Outcome"/>
        <rdfs:comment xml:lang="en">An Evaluation Outcome can have any number of [contributions](../entities/Contribution_to_Evaluation_Outcome.md) that helped it arise.</rdfs:comment>
    </owl:ObjectProperty>
    


    <!-- https://w3id.org/cerif2/Evaluation_Outcome#isAnEvaluationOutcomeOf -->


    <owl:ObjectProperty rdf:about="https://w3id.org/cerif2/Evaluation_Outcome#isAnEvaluationOutcomeOf">
        <owl:inverseOf rdf:resource="https://w3id.org/cerif2/Resource_Request#hasEvaluationOutcome"/>
        <rdfs:domain rdf:resource="https://w3id.org/cerif2/Evaluation_Outcome"/>
        <rdfs:range rdf:resource="https://w3id.org/cerif2/Resource_Request"/>
        <rdfs:comment xml:lang="en">An Evaluation outcome might be a result of the [Resource Request](../entities/Resource_Request.md) evaluation process.</rdfs:comment>
    </owl:ObjectProperty>
    


    <!-- https://w3id.org/cerif2/Evaluation_Outcome#providesBasisFor -->


    <owl:ObjectProperty rdf:about="https://w3id.org/cerif2/Evaluation_Outcome#providesBasisFor">
        <rdfs:domain rdf:resource="https://w3id.org/cerif2/Evaluation_Outcome"/>
        <rdfs:range rdf:resource="https://w3id.org/cerif2/Decision"/>
        <rdfs:comment xml:lang="en">Conclusions from evaluation process can be a basis for final [Decision](../entities/Decision.md).</rdfs:comment>
    </owl:ObjectProperty>
    


    <!-- https://w3id.org/cerif2/Event#awardedBy -->


    <owl:ObjectProperty rdf:about="https://w3id.org/cerif2/Event#awardedBy">
        <owl:inverseOf rdf:resource="https://w3id.org/cerif2/Prize_Award#awardedForAnEvent"/>
        <rdfs:domain rdf:resource="https://w3id.org/cerif2/Event"/>
        <rdfs:range rdf:resource="https://w3id.org/cerif2/Prize_Award"/>
        <rdfs:comment xml:lang="en">An Event can be awarded by a [Prize Award](../entities/Prize_Award.md).</rdfs:comment>
    </owl:ObjectProperty>
    


    <!-- https://w3id.org/cerif2/Event#belongsToSeries -->


    <owl:ObjectProperty rdf:about="https://w3id.org/cerif2/Event#belongsToSeries">
        <owl:inverseOf rdf:resource="https://w3id.org/cerif2/Event_Series#hasInstances"/>
        <rdfs:domain rdf:resource="https://w3id.org/cerif2/Event"/>
        <rdfs:range rdf:resource="https://w3id.org/cerif2/Event_Series"/>
        <rdfs:comment xml:lang="en">An Event can be an instance of [Event Series](../entities/Event_Series.md).</rdfs:comment>
    </owl:ObjectProperty>
    


    <!-- https://w3id.org/cerif2/Event#dateRange -->


    <owl:ObjectProperty rdf:about="https://w3id.org/cerif2/Event#dateRange">
        <rdfs:domain rdf:resource="https://w3id.org/cerif2/Event"/>
        <rdfs:range rdf:resource="https://w3id.org/cerif2/Date_Range"/>
    </owl:ObjectProperty>
    


    <!-- https://w3id.org/cerif2/Event#hasContribution -->


    <owl:ObjectProperty rdf:about="https://w3id.org/cerif2/Event#hasContribution">
        <rdfs:domain rdf:resource="https://w3id.org/cerif2/Event"/>
        <rdfs:range rdf:resource="https://w3id.org/cerif2/Contribution_to_Event"/>
        <rdfs:comment xml:lang="en">An Event can have any number of [contributions](../entities/Contribution_to_Event.md) that helped it take place or arise.</rdfs:comment>
    </owl:ObjectProperty>
    


    <!-- https://w3id.org/cerif2/Event_Identifier#isAssignedTo -->


    <owl:ObjectProperty rdf:about="https://w3id.org/cerif2/Event_Identifier#isAssignedTo">
        <owl:inverseOf rdf:resource="https://w3id.org/cerif2/Event_Series#hasIdentifier"/>
        <rdfs:domain rdf:resource="https://w3id.org/cerif2/Event_Identifier"/>
        <rdfs:range rdf:resource="https://w3id.org/cerif2/Event_Series"/>
        <rdfs:comment xml:lang="en">An Event Identifier can be assigned to an [Event Series](../entities/Event_Series.md).</rdfs:comment>
    </owl:ObjectProperty>
    


    <!-- https://w3id.org/cerif2/Event_Series#hasIdentifier -->


    <owl:ObjectProperty rdf:about="https://w3id.org/cerif2/Event_Series#hasIdentifier">
        <rdfs:domain rdf:resource="https://w3id.org/cerif2/Event_Series"/>
        <rdfs:range rdf:resource="https://w3id.org/cerif2/Event_Identifier"/>
        <rdfs:comment xml:lang="en">An Event Series can have any number of [Event Identifiers](../entities/Event_Identifier.md).</rdfs:comment>
    </owl:ObjectProperty>
    


    <!-- https://w3id.org/cerif2/Event_Series#hasInstances -->


    <owl:ObjectProperty rdf:about="https://w3id.org/cerif2/Event_Series#hasInstances">
        <rdfs:domain rdf:resource="https://w3id.org/cerif2/Event_Series"/>
        <rdfs:range rdf:resource="https://w3id.org/cerif2/Event"/>
        <rdfs:comment xml:lang="en">An Event Series has list of [Event](../entities/Event.md) instances which have been organized.</rdfs:comment>
    </owl:ObjectProperty>
    


    <!-- https://w3id.org/cerif2/Expertise_and_Skills#isPossessedThrough -->


    <owl:ObjectProperty rdf:about="https://w3id.org/cerif2/Expertise_and_Skills#isPossessedThrough">
        <owl:inverseOf rdf:resource="https://w3id.org/cerif2/Expertise_and_Skills_Possession#possesses"/>
        <rdfs:domain rdf:resource="https://w3id.org/cerif2/Expertise_and_Skills"/>
        <rdfs:range rdf:resource="https://w3id.org/cerif2/Expertise_and_Skills_Possession"/>
        <rdfs:comment xml:lang="en">A Expertise and Skills can be possessed in any number of [Expertise and Skills Possessions](../entities/Expertise_and_Skills_Possession.md).</rdfs:comment>
    </owl:ObjectProperty>
    


    <!-- https://w3id.org/cerif2/Expertise_and_Skills#isUsedAsAResource -->


    <owl:ObjectProperty rdf:about="https://w3id.org/cerif2/Expertise_and_Skills#isUsedAsAResource">
        <rdfs:domain rdf:resource="https://w3id.org/cerif2/Expertise_and_Skills"/>
        <rdfs:range rdf:resource="https://w3id.org/cerif2/Expertise_and_Time_and_Effort"/>
        <rdfs:comment xml:lang="en">A Expertise and Skills can be used as a resource in any number of [Expertise and Time and Effort](../entities/Expertise_and_Time_and_Effort.md).</rdfs:comment>
    </owl:ObjectProperty>
    


    <!-- https://w3id.org/cerif2/Expertise_and_Skills_Possession#byAgent -->


    <owl:ObjectProperty rdf:about="https://w3id.org/cerif2/Expertise_and_Skills_Possession#byAgent">
        <rdfs:domain rdf:resource="https://w3id.org/cerif2/Expertise_and_Skills_Possession"/>
        <rdfs:range rdf:resource="https://w3id.org/cerif2/Agent"/>
        <rdfs:comment xml:lang="en">An Expertise and Skills Possession references the [Agent](../entities/Agent.md) who posesses the [Expertise and Skills](../entities/Expertise_and_Skills.md).</rdfs:comment>
    </owl:ObjectProperty>
    


    <!-- https://w3id.org/cerif2/Expertise_and_Skills_Possession#isEvidencedBy -->


    <owl:ObjectProperty rdf:about="https://w3id.org/cerif2/Expertise_and_Skills_Possession#isEvidencedBy">
        <rdfs:domain rdf:resource="https://w3id.org/cerif2/Expertise_and_Skills_Possession"/>
        <rdfs:range rdf:resource="https://w3id.org/cerif2/Document"/>
        <rdfs:comment xml:lang="en">An Expertise and Skills Possession can be evidenced by any number of [Documents](../entities/Document.md).</rdfs:comment>
    </owl:ObjectProperty>
    


    <!-- https://w3id.org/cerif2/Expertise_and_Skills_Possession#possesses -->


    <owl:ObjectProperty rdf:about="https://w3id.org/cerif2/Expertise_and_Skills_Possession#possesses">
        <rdfs:domain rdf:resource="https://w3id.org/cerif2/Expertise_and_Skills_Possession"/>
        <rdfs:range rdf:resource="https://w3id.org/cerif2/Expertise_and_Skills"/>
        <rdfs:comment xml:lang="en">An Expertise and Skills Possession references the [Expertise and Skills](../entities/Expertise_and_Skills.md) that the Agent possesses.</rdfs:comment>
    </owl:ObjectProperty>
    


    <!-- https://w3id.org/cerif2/Expertise_and_Time_and_Effort#byAgent -->


    <owl:ObjectProperty rdf:about="https://w3id.org/cerif2/Expertise_and_Time_and_Effort#byAgent">
        <rdfs:domain rdf:resource="https://w3id.org/cerif2/Expertise_and_Time_and_Effort"/>
        <rdfs:range rdf:resource="https://w3id.org/cerif2/Agent"/>
        <rdfs:comment xml:lang="en">An Expertise and Time and Effort references the [Agent](../entities/Agent.md) whose expertise, time and effort it would be.</rdfs:comment>
    </owl:ObjectProperty>
    


    <!-- https://w3id.org/cerif2/Funding#amount -->


    <owl:ObjectProperty rdf:about="https://w3id.org/cerif2/Funding#amount">
        <rdfs:domain rdf:resource="https://w3id.org/cerif2/Funding"/>
        <rdfs:range rdf:resource="https://w3id.org/cerif2/Monetary_Amount"/>
    </owl:ObjectProperty>
    


    <!-- https://w3id.org/cerif2/Funding#covers -->


    <owl:ObjectProperty rdf:about="https://w3id.org/cerif2/Funding#covers">
        <owl:inverseOf rdf:resource="https://w3id.org/cerif2/Project#fundedBy"/>
        <rdfs:domain rdf:resource="https://w3id.org/cerif2/Funding"/>
        <rdfs:range rdf:resource="https://w3id.org/cerif2/Project"/>
        <rdfs:comment xml:lang="en">A Funding can cover any number of [Projects](../entities/Project.md) that help it happen.</rdfs:comment>
    </owl:ObjectProperty>
    


    <!-- https://w3id.org/cerif2/Group#hasPart -->


    <owl:ObjectProperty rdf:about="https://w3id.org/cerif2/Group#hasPart">
        <owl:inverseOf rdf:resource="https://w3id.org/cerif2/Group#isPartOf"/>
        <rdfs:domain rdf:resource="https://w3id.org/cerif2/Group"/>
        <rdfs:range rdf:resource="https://w3id.org/cerif2/Group"/>
        <rdfs:comment xml:lang="en">A Group can have any number of parts, instances of [Group](../entities/Group.md).</rdfs:comment>
    </owl:ObjectProperty>
    


    <!-- https://w3id.org/cerif2/Group#isPartOf -->


    <owl:ObjectProperty rdf:about="https://w3id.org/cerif2/Group#isPartOf">
        <rdfs:domain rdf:resource="https://w3id.org/cerif2/Group"/>
        <rdfs:range rdf:resource="https://w3id.org/cerif2/Group"/>
        <rdfs:comment xml:lang="en">A Group can be part of any number of other [Groups](../entities/Group.md).</rdfs:comment>
    </owl:ObjectProperty>
    


    <!-- https://w3id.org/cerif2/Group_or_Organisation_Unit#hasInvolvement -->


    <owl:ObjectProperty rdf:about="https://w3id.org/cerif2/Group_or_Organisation_Unit#hasInvolvement">
        <owl:inverseOf rdf:resource="https://w3id.org/cerif2/Involvement#involvesActorIn"/>
        <rdfs:domain rdf:resource="https://w3id.org/cerif2/Group_or_Organisation_Unit"/>
        <rdfs:range rdf:resource="https://w3id.org/cerif2/Involvement"/>
        <rdfs:comment xml:lang="en">A Group or Organisation Unit can have any number of [Involvements](../entities/Involvement.md), which involve [Agents](../entities/Agent.md) in it.</rdfs:comment>
    </owl:ObjectProperty>
    


    <!-- https://w3id.org/cerif2/Infrastructure#hasContribution -->


    <owl:ObjectProperty rdf:about="https://w3id.org/cerif2/Infrastructure#hasContribution">
        <rdfs:domain rdf:resource="https://w3id.org/cerif2/Infrastructure"/>
        <rdfs:range rdf:resource="https://w3id.org/cerif2/Contribution_to_Infrastructure"/>
        <rdfs:comment xml:lang="en">An Infrastructure can have any number of [contributions](../entities/Contribution_to_Infrastructure.md) that helped it arise, keep or develop.</rdfs:comment>
    </owl:ObjectProperty>
    


    <!-- https://w3id.org/cerif2/Involvement#hasPart -->


    <owl:ObjectProperty rdf:about="https://w3id.org/cerif2/Involvement#hasPart">
        <owl:inverseOf rdf:resource="https://w3id.org/cerif2/Involvement#isPartOf"/>
        <rdfs:domain rdf:resource="https://w3id.org/cerif2/Involvement"/>
        <rdfs:range rdf:resource="https://w3id.org/cerif2/Involvement"/>
        <rdfs:comment xml:lang="en">An Involvement can have any number of part [Involvements](../entities/Involvement.md).</rdfs:comment>
    </owl:ObjectProperty>
    


    <!-- https://w3id.org/cerif2/Involvement#involvesActorIn -->


    <owl:ObjectProperty rdf:about="https://w3id.org/cerif2/Involvement#involvesActorIn">
        <rdfs:domain rdf:resource="https://w3id.org/cerif2/Involvement"/>
        <rdfs:range rdf:resource="https://w3id.org/cerif2/Group_or_Organisation_Unit"/>
        <rdfs:comment xml:lang="en">A Involvement specifies that the *actor* Agent is involved in a [Group or Organisation Units](../entities/Group_or_Organisation_Unit.md).</rdfs:comment>
    </owl:ObjectProperty>
    


    <!-- https://w3id.org/cerif2/Involvement#isPartOf -->


    <owl:ObjectProperty rdf:about="https://w3id.org/cerif2/Involvement#isPartOf">
        <rdfs:domain rdf:resource="https://w3id.org/cerif2/Involvement"/>
        <rdfs:range rdf:resource="https://w3id.org/cerif2/Involvement"/>
        <rdfs:comment xml:lang="en">An Involvement can be part of any number of other [Involvements](../entities/Involvement.md).</rdfs:comment>
    </owl:ObjectProperty>
    


    <!-- https://w3id.org/cerif2/Involvement#isTheFoundationFor -->


    <owl:ObjectProperty rdf:about="https://w3id.org/cerif2/Involvement#isTheFoundationFor">
        <rdfs:domain rdf:resource="https://w3id.org/cerif2/Involvement"/>
        <rdfs:range rdf:resource="https://w3id.org/cerif2/Affiliation_Statement"/>
        <rdfs:comment xml:lang="en">An Involvement can be foundation for an [Affiliation Statement](../entities/Affiliation_Statement.md).</rdfs:comment>
    </owl:ObjectProperty>
    


    <!-- https://w3id.org/cerif2/Involvement#position -->


    <owl:ObjectProperty rdf:about="https://w3id.org/cerif2/Involvement#position">
        <rdfs:domain rdf:resource="https://w3id.org/cerif2/Involvement"/>
        <rdfs:range rdf:resource="https://w3id.org/cerif2/Position"/>
    </owl:ObjectProperty>
    


    <!-- https://w3id.org/cerif2/Organisation_Unit#hasPart -->


    <owl:ObjectProperty rdf:about="https://w3id.org/cerif2/Organisation_Unit#hasPart">
        <owl:inverseOf rdf:resource="https://w3id.org/cerif2/Organisation_Unit#isPartOf"/>
        <rdfs:domain rdf:resource="https://w3id.org/cerif2/Organisation_Unit"/>
        <rdfs:range rdf:resource="https://w3id.org/cerif2/Organisation_Unit"/>
        <rdfs:comment xml:lang="en">An Organisation Unit can have any number of parts, instances of [Organisation Unit](../entities/Organisation_Unit.md).</rdfs:comment>
    </owl:ObjectProperty>
    


    <!-- https://w3id.org/cerif2/Organisation_Unit#isPartOf -->


    <owl:ObjectProperty rdf:about="https://w3id.org/cerif2/Organisation_Unit#isPartOf">
        <rdfs:domain rdf:resource="https://w3id.org/cerif2/Organisation_Unit"/>
        <rdfs:range rdf:resource="https://w3id.org/cerif2/Organisation_Unit"/>
        <rdfs:comment xml:lang="en">An Organisation Unit can be part of any number of other [Organisation Units](../entities/Organisation_Unit.md).</rdfs:comment>
    </owl:ObjectProperty>
    


    <!-- https://w3id.org/cerif2/Organisation_Unit#isTheInstitutionIn -->


    <owl:ObjectProperty rdf:about="https://w3id.org/cerif2/Organisation_Unit#isTheInstitutionIn">
        <rdfs:domain rdf:resource="https://w3id.org/cerif2/Organisation_Unit"/>
        <rdfs:range rdf:resource="https://w3id.org/cerif2/Affiliation_Statement"/>
        <rdfs:comment xml:lang="en">An Organisation Unit can be the institution in any number of [Affiliation Statements](../entities/Affiliation_Statement.md).</rdfs:comment>
    </owl:ObjectProperty>
    


    <!-- https://w3id.org/cerif2/Organisation_Unit#isTheOrganisationUnitIn -->


    <owl:ObjectProperty rdf:about="https://w3id.org/cerif2/Organisation_Unit#isTheOrganisationUnitIn">
        <rdfs:domain rdf:resource="https://w3id.org/cerif2/Organisation_Unit"/>
        <rdfs:range rdf:resource="https://w3id.org/cerif2/Affiliation_Statement"/>
        <rdfs:comment xml:lang="en">A Organisation Unit can is the organisation unit in any number of [Affiliation Statements](../entities/Affiliation_Statement.md).</rdfs:comment>
    </owl:ObjectProperty>
    


    <!-- https://w3id.org/cerif2/Person#alternateNames -->


    <owl:ObjectProperty rdf:about="https://w3id.org/cerif2/Person#alternateNames">
        <rdfs:domain rdf:resource="https://w3id.org/cerif2/Person"/>
        <rdfs:range rdf:resource="https://w3id.org/cerif2/Person_Name"/>
    </owl:ObjectProperty>
    


    <!-- https://w3id.org/cerif2/Person#isThePersonIn -->


    <owl:ObjectProperty rdf:about="https://w3id.org/cerif2/Person#isThePersonIn">
        <rdfs:domain rdf:resource="https://w3id.org/cerif2/Person"/>
        <rdfs:range rdf:resource="https://w3id.org/cerif2/Affiliation_Statement"/>
        <rdfs:comment xml:lang="en">A Person can be the person in any number of [Affiliation Statements](../entities/Affiliation_Statement.md).</rdfs:comment>
    </owl:ObjectProperty>
    


    <!-- https://w3id.org/cerif2/Person#name -->


    <owl:ObjectProperty rdf:about="https://w3id.org/cerif2/Person#name">
        <rdfs:domain rdf:resource="https://w3id.org/cerif2/Person"/>
        <rdfs:range rdf:resource="https://w3id.org/cerif2/Person_Name"/>
    </owl:ObjectProperty>
    


    <!-- https://w3id.org/cerif2/Physical_Address#country -->


    <owl:ObjectProperty rdf:about="https://w3id.org/cerif2/Physical_Address#country">
        <rdfs:domain rdf:resource="https://w3id.org/cerif2/Physical_Address"/>
        <rdfs:range rdf:resource="https://w3id.org/cerif2/Country"/>
    </owl:ObjectProperty>
    


    <!-- https://w3id.org/cerif2/Postal_Address#physicalAddress -->


    <owl:ObjectProperty rdf:about="https://w3id.org/cerif2/Postal_Address#physicalAddress">
        <rdfs:domain rdf:resource="https://w3id.org/cerif2/Postal_Address"/>
        <rdfs:range rdf:resource="https://w3id.org/cerif2/Physical_Address"/>
    </owl:ObjectProperty>
    


    <!-- https://w3id.org/cerif2/Prize#hasContribution -->


    <owl:ObjectProperty rdf:about="https://w3id.org/cerif2/Prize#hasContribution">
        <rdfs:domain rdf:resource="https://w3id.org/cerif2/Prize"/>
        <rdfs:range rdf:resource="https://w3id.org/cerif2/Contribution_to_Prize"/>
        <rdfs:comment xml:lang="en">A Prize can have any number of [contributions](../entities/Contribution_to_Prize.md) that help it arise or continue.</rdfs:comment>
    </owl:ObjectProperty>
    


    <!-- https://w3id.org/cerif2/Prize#isAwardedAs -->


    <owl:ObjectProperty rdf:about="https://w3id.org/cerif2/Prize#isAwardedAs">
        <owl:inverseOf rdf:resource="https://w3id.org/cerif2/Prize_Award#awards"/>
        <rdfs:domain rdf:resource="https://w3id.org/cerif2/Prize"/>
        <rdfs:range rdf:resource="https://w3id.org/cerif2/Prize_Award"/>
        <rdfs:comment xml:lang="en">A Prize can be awarded through any number of [Prize Awards](../entities/Prize_Award.md).</rdfs:comment>
    </owl:ObjectProperty>
    


    <!-- https://w3id.org/cerif2/Prize_Award#awardedByWhom -->


    <owl:ObjectProperty rdf:about="https://w3id.org/cerif2/Prize_Award#awardedByWhom">
        <rdfs:domain rdf:resource="https://w3id.org/cerif2/Prize_Award"/>
        <rdfs:range rdf:resource="https://w3id.org/cerif2/Event"/>
        <rdfs:comment xml:lang="en">A Prize can be awarded by any number of [Agents](../entities/Agent.md).</rdfs:comment>
    </owl:ObjectProperty>
    


    <!-- https://w3id.org/cerif2/Prize_Award#awardedForADocument -->


    <owl:ObjectProperty rdf:about="https://w3id.org/cerif2/Prize_Award#awardedForADocument">
        <rdfs:domain rdf:resource="https://w3id.org/cerif2/Prize_Award"/>
        <rdfs:range rdf:resource="https://w3id.org/cerif2/Document"/>
        <rdfs:comment xml:lang="en">A Prize can be awarded for a [Document](../entities/Document.md).</rdfs:comment>
    </owl:ObjectProperty>
    


    <!-- https://w3id.org/cerif2/Prize_Award#awardedForAProject -->


    <owl:ObjectProperty rdf:about="https://w3id.org/cerif2/Prize_Award#awardedForAProject">
        <owl:inverseOf rdf:resource="https://w3id.org/cerif2/Project#awardedBy"/>
        <rdfs:domain rdf:resource="https://w3id.org/cerif2/Prize_Award"/>
        <rdfs:range rdf:resource="https://w3id.org/cerif2/Project"/>
        <rdfs:comment xml:lang="en">A Prize can be awarded for a [Project](../entities/Project.md).</rdfs:comment>
    </owl:ObjectProperty>
    


    <!-- https://w3id.org/cerif2/Prize_Award#awardedForAnEvent -->


    <owl:ObjectProperty rdf:about="https://w3id.org/cerif2/Prize_Award#awardedForAnEvent">
        <rdfs:domain rdf:resource="https://w3id.org/cerif2/Prize_Award"/>
        <rdfs:range rdf:resource="https://w3id.org/cerif2/Event"/>
        <rdfs:comment xml:lang="en">A Prize can be awarded for an [Event](../entities/Event.md).</rdfs:comment>
    </owl:ObjectProperty>
    


    <!-- https://w3id.org/cerif2/Prize_Award#awards -->


    <owl:ObjectProperty rdf:about="https://w3id.org/cerif2/Prize_Award#awards">
        <rdfs:domain rdf:resource="https://w3id.org/cerif2/Prize_Award"/>
        <rdfs:range rdf:resource="https://w3id.org/cerif2/Prize"/>
        <rdfs:comment xml:lang="en">A Prize Award awards a specific [Prize](../entities/Prize.md).</rdfs:comment>
    </owl:ObjectProperty>
    


    <!-- https://w3id.org/cerif2/Prize_Award#hasContribution -->


    <owl:ObjectProperty rdf:about="https://w3id.org/cerif2/Prize_Award#hasContribution">
        <rdfs:domain rdf:resource="https://w3id.org/cerif2/Prize_Award"/>
        <rdfs:range rdf:resource="https://w3id.org/cerif2/Contribution_to_Prize_Award"/>
        <rdfs:comment xml:lang="en">A Prize Award can have any number of [contributions](../entities/Contribution_to_Prize_Award.md) that help its organization.</rdfs:comment>
    </owl:ObjectProperty>
    


    <!-- https://w3id.org/cerif2/Prize_Award#hasRecipient -->


    <owl:ObjectProperty rdf:about="https://w3id.org/cerif2/Prize_Award#hasRecipient">
        <rdfs:domain rdf:resource="https://w3id.org/cerif2/Prize_Award"/>
        <rdfs:range rdf:resource="https://w3id.org/cerif2/Agent"/>
        <rdfs:comment xml:lang="en">A Prize Award can have any number of recipients, instances of [Agent](../entities/Agent.md).</rdfs:comment>
    </owl:ObjectProperty>
    


    <!-- https://w3id.org/cerif2/Project#awardedBy -->


    <owl:ObjectProperty rdf:about="https://w3id.org/cerif2/Project#awardedBy">
        <rdfs:domain rdf:resource="https://w3id.org/cerif2/Project"/>
        <rdfs:range rdf:resource="https://w3id.org/cerif2/Prize_Award"/>
        <rdfs:comment xml:lang="en">A Project can be awarded by a [Prize Award](../entities/Prize_Award.md).</rdfs:comment>
    </owl:ObjectProperty>
    


    <!-- https://w3id.org/cerif2/Project#fundedBy -->


    <owl:ObjectProperty rdf:about="https://w3id.org/cerif2/Project#fundedBy">
        <rdfs:domain rdf:resource="https://w3id.org/cerif2/Project"/>
        <rdfs:range rdf:resource="https://w3id.org/cerif2/Funding"/>
        <rdfs:comment xml:lang="en">A Project can have any number of [Fundings](../entities/Funding.md) that help it happen.</rdfs:comment>
    </owl:ObjectProperty>
    


    <!-- https://w3id.org/cerif2/Project#hasContribution -->


    <owl:ObjectProperty rdf:about="https://w3id.org/cerif2/Project#hasContribution">
        <rdfs:domain rdf:resource="https://w3id.org/cerif2/Project"/>
        <rdfs:range rdf:resource="https://w3id.org/cerif2/Contribution_to_Project"/>
        <rdfs:comment xml:lang="en">A Project can have any number of [contributions](../entities/Contribution_to_Project.md) that help it happen.</rdfs:comment>
    </owl:ObjectProperty>
    


    <!-- https://w3id.org/cerif2/Project#hasPart -->


    <owl:ObjectProperty rdf:about="https://w3id.org/cerif2/Project#hasPart">
        <owl:inverseOf rdf:resource="https://w3id.org/cerif2/Project#isPartOf"/>
        <rdfs:domain rdf:resource="https://w3id.org/cerif2/Project"/>
        <rdfs:range rdf:resource="https://w3id.org/cerif2/Project"/>
        <rdfs:comment xml:lang="en">A Project Unit can have any number of parts, instances of [Project](../entities/Project.md).</rdfs:comment>
    </owl:ObjectProperty>
    


    <!-- https://w3id.org/cerif2/Project#isPartOf -->


    <owl:ObjectProperty rdf:about="https://w3id.org/cerif2/Project#isPartOf">
        <rdfs:domain rdf:resource="https://w3id.org/cerif2/Project"/>
        <rdfs:range rdf:resource="https://w3id.org/cerif2/Project"/>
        <rdfs:comment xml:lang="en">A Project Unit (sub-project/work package/task) can be part of the other [Project unit](../entities/Project.md).</rdfs:comment>
    </owl:ObjectProperty>
    


    <!-- https://w3id.org/cerif2/Publication_Channel#contains -->


    <owl:ObjectProperty rdf:about="https://w3id.org/cerif2/Publication_Channel#contains">
        <rdfs:domain rdf:resource="https://w3id.org/cerif2/Publication_Channel"/>
        <rdfs:range rdf:resource="https://w3id.org/cerif2/Document_Publication"/>
        <rdfs:comment xml:lang="en">A Publication Channel contains any number of [Document Publications](../entities/Document_Publication.md). [Contents Location](../datatypes/Contents_Location.md) can be attached to such an association.</rdfs:comment>
    </owl:ObjectProperty>
    


    <!-- https://w3id.org/cerif2/Resource#hasIdentifier -->


    <owl:ObjectProperty rdf:about="https://w3id.org/cerif2/Resource#hasIdentifier">
        <owl:inverseOf rdf:resource="https://w3id.org/cerif2/Resource_Identifier#isAssignedTo"/>
        <rdfs:domain rdf:resource="https://w3id.org/cerif2/Resource"/>
        <rdfs:range rdf:resource="https://w3id.org/cerif2/Resource_Identifier"/>
        <rdfs:comment xml:lang="en">A Resource can have any number of [identifiers](../entities/Resource_Identifier.md).</rdfs:comment>
    </owl:ObjectProperty>
    


    <!-- https://w3id.org/cerif2/Resource#hasPart -->


    <owl:ObjectProperty rdf:about="https://w3id.org/cerif2/Resource#hasPart">
        <owl:inverseOf rdf:resource="https://w3id.org/cerif2/Resource#isPartOf"/>
        <rdfs:domain rdf:resource="https://w3id.org/cerif2/Resource"/>
        <rdfs:range rdf:resource="https://w3id.org/cerif2/Resource"/>
        <rdfs:comment xml:lang="en">A Resource can have any number of other [Resources](../entities/Resource.md) as parts.</rdfs:comment>
    </owl:ObjectProperty>
    


    <!-- https://w3id.org/cerif2/Resource#isOfferedIn -->


    <owl:ObjectProperty rdf:about="https://w3id.org/cerif2/Resource#isOfferedIn">
        <owl:inverseOf rdf:resource="https://w3id.org/cerif2/Resource_Offer#offers"/>
        <rdfs:domain rdf:resource="https://w3id.org/cerif2/Resource"/>
        <rdfs:range rdf:resource="https://w3id.org/cerif2/Resource_Offer"/>
        <rdfs:comment xml:lang="en">A Resource can be offered in any number of [Resource Offers](../entities/Resource_Offer.md).</rdfs:comment>
    </owl:ObjectProperty>
    


    <!-- https://w3id.org/cerif2/Resource#isPartOf -->


    <owl:ObjectProperty rdf:about="https://w3id.org/cerif2/Resource#isPartOf">
        <rdfs:domain rdf:resource="https://w3id.org/cerif2/Resource"/>
        <rdfs:range rdf:resource="https://w3id.org/cerif2/Resource"/>
        <rdfs:comment xml:lang="en">A Resource can be part of any number of other [Resources](../entities/Resource.md).</rdfs:comment>
    </owl:ObjectProperty>
    


    <!-- https://w3id.org/cerif2/Resource#isProvidedBy -->


    <owl:ObjectProperty rdf:about="https://w3id.org/cerif2/Resource#isProvidedBy">
        <rdfs:domain rdf:resource="https://w3id.org/cerif2/Resource"/>
        <rdfs:range rdf:resource="https://w3id.org/cerif2/Contribution_Statement"/>
        <rdfs:comment xml:lang="en">A Resource can be provided in any number of [Contribution Statements](../entities/Contribution_Statement.md).</rdfs:comment>
    </owl:ObjectProperty>
    


    <!-- https://w3id.org/cerif2/Resource#isRequestedIn -->


    <owl:ObjectProperty rdf:about="https://w3id.org/cerif2/Resource#isRequestedIn">
        <owl:inverseOf rdf:resource="https://w3id.org/cerif2/Resource_Request#requests"/>
        <rdfs:domain rdf:resource="https://w3id.org/cerif2/Resource"/>
        <rdfs:range rdf:resource="https://w3id.org/cerif2/Resource_Request"/>
        <rdfs:comment xml:lang="en">A Resource can be requested in any number of [Resource Requests](../entities/Resource_Request.md).</rdfs:comment>
    </owl:ObjectProperty>
    


    <!-- https://w3id.org/cerif2/Resource#isUsedIn -->


    <owl:ObjectProperty rdf:about="https://w3id.org/cerif2/Resource#isUsedIn">
        <owl:inverseOf rdf:resource="https://w3id.org/cerif2/Resource_Usage_Statement#uses"/>
        <rdfs:domain rdf:resource="https://w3id.org/cerif2/Resource"/>
        <rdfs:range rdf:resource="https://w3id.org/cerif2/Resource_Usage_Statement"/>
        <rdfs:comment xml:lang="en">When a Resource is used, the usage can be detailed in [Resource Usage Statements](../entities/Resource_Usage_Statement.md). For instance, a funding, a dataset or a piece of equipment can be used in producing a journal article.</rdfs:comment>
    </owl:ObjectProperty>
    


    <!-- https://w3id.org/cerif2/Resource_Identifier#isAssignedTo -->


    <owl:ObjectProperty rdf:about="https://w3id.org/cerif2/Resource_Identifier#isAssignedTo">
        <rdfs:domain rdf:resource="https://w3id.org/cerif2/Resource_Identifier"/>
        <rdfs:range rdf:resource="https://w3id.org/cerif2/Resource"/>
        <rdfs:comment xml:lang="en">A Resource Identifier can be assigned to a [Resource](../entities/Resource.md).</rdfs:comment>
    </owl:ObjectProperty>
    


    <!-- https://w3id.org/cerif2/Resource_Offer#hasCondition -->


    <owl:ObjectProperty rdf:about="https://w3id.org/cerif2/Resource_Offer#hasCondition">
        <rdfs:domain rdf:resource="https://w3id.org/cerif2/Resource_Offer"/>
        <rdfs:range rdf:resource="https://w3id.org/cerif2/Condition"/>
        <rdfs:comment xml:lang="en">A Resource Offer can have any number of [Conditions](../entities/Condition.md) that must be satisfied for the Resource Offer to be applicable.</rdfs:comment>
    </owl:ObjectProperty>
    


    <!-- https://w3id.org/cerif2/Resource_Offer#isDescribedBy -->


    <owl:ObjectProperty rdf:about="https://w3id.org/cerif2/Resource_Offer#isDescribedBy">
        <rdfs:domain rdf:resource="https://w3id.org/cerif2/Resource_Offer"/>
        <rdfs:range rdf:resource="https://w3id.org/cerif2/Document"/>
        <rdfs:comment xml:lang="en">A Resource Offer can be described by any number of [Documents](../entities/Document.md).</rdfs:comment>
    </owl:ObjectProperty>
    


    <!-- https://w3id.org/cerif2/Resource_Offer#isSolicitedBy -->


    <owl:ObjectProperty rdf:about="https://w3id.org/cerif2/Resource_Offer#isSolicitedBy">
        <rdfs:domain rdf:resource="https://w3id.org/cerif2/Resource_Offer"/>
        <rdfs:range rdf:resource="https://w3id.org/cerif2/Agent"/>
        <rdfs:comment xml:lang="en">A Resource Offer is solicited by an [Agent](../entities/Agent.md).</rdfs:comment>
    </owl:ObjectProperty>
    


    <!-- https://w3id.org/cerif2/Resource_Offer#offers -->


    <owl:ObjectProperty rdf:about="https://w3id.org/cerif2/Resource_Offer#offers">
        <rdfs:domain rdf:resource="https://w3id.org/cerif2/Resource_Offer"/>
        <rdfs:range rdf:resource="https://w3id.org/cerif2/Resource"/>
        <rdfs:comment xml:lang="en">A Resource Offer specifies the [Resource](../entities/Resource.md) that is the subject of the offer.</rdfs:comment>
    </owl:ObjectProperty>
    


    <!-- https://w3id.org/cerif2/Resource_Request#hasAddressee -->


    <owl:ObjectProperty rdf:about="https://w3id.org/cerif2/Resource_Request#hasAddressee">
        <rdfs:domain rdf:resource="https://w3id.org/cerif2/Resource_Request"/>
        <rdfs:range rdf:resource="https://w3id.org/cerif2/Agent"/>
        <rdfs:comment xml:lang="en">A Resource Request always references its addressee, the [Agent](../entities/Agent.md) that is expected to consider the resource request. (Note the role can be called differently in specific contexts.)</rdfs:comment>
    </owl:ObjectProperty>
    


    <!-- https://w3id.org/cerif2/Resource_Request#hasDecision -->


    <owl:ObjectProperty rdf:about="https://w3id.org/cerif2/Resource_Request#hasDecision">
        <rdfs:domain rdf:resource="https://w3id.org/cerif2/Resource_Request"/>
        <rdfs:range rdf:resource="https://w3id.org/cerif2/Decision"/>
        <rdfs:comment xml:lang="en">A Resource Request can have a [Decision](../entities/Decision.md) about accepting or refusing request made by addressee.</rdfs:comment>
    </owl:ObjectProperty>
    


    <!-- https://w3id.org/cerif2/Resource_Request#hasEvaluationOutcome -->


    <owl:ObjectProperty rdf:about="https://w3id.org/cerif2/Resource_Request#hasEvaluationOutcome">
        <rdfs:domain rdf:resource="https://w3id.org/cerif2/Resource_Request"/>
        <rdfs:range rdf:resource="https://w3id.org/cerif2/Evaluation_Outcome"/>
        <rdfs:comment xml:lang="en">A Resource Request can have some kind of process which results in an [Evaluation Outcome](../entities/Evaluation_Outcome.md).</rdfs:comment>
    </owl:ObjectProperty>
    


    <!-- https://w3id.org/cerif2/Resource_Request#hasRequester -->


    <owl:ObjectProperty rdf:about="https://w3id.org/cerif2/Resource_Request#hasRequester">
        <rdfs:domain rdf:resource="https://w3id.org/cerif2/Resource_Request"/>
        <rdfs:range rdf:resource="https://w3id.org/cerif2/Agent"/>
        <rdfs:comment xml:lang="en">A Resource Request always has the requester: the [Agent](../entities/Agent.md) that is requesting a resource. (Note that the role can be called differently in specific contexts, for instance applicant.)</rdfs:comment>
    </owl:ObjectProperty>
    


    <!-- https://w3id.org/cerif2/Resource_Request#isDescribedBy -->


    <owl:ObjectProperty rdf:about="https://w3id.org/cerif2/Resource_Request#isDescribedBy">
        <rdfs:domain rdf:resource="https://w3id.org/cerif2/Resource_Request"/>
        <rdfs:range rdf:resource="https://w3id.org/cerif2/Document"/>
        <rdfs:comment xml:lang="en">A Resource Request can optionally reference its contents, the [Document](../entities/Document.md) that details the resource request.</rdfs:comment>
    </owl:ObjectProperty>
    


    <!-- https://w3id.org/cerif2/Resource_Request#requests -->


    <owl:ObjectProperty rdf:about="https://w3id.org/cerif2/Resource_Request#requests">
        <rdfs:domain rdf:resource="https://w3id.org/cerif2/Resource_Request"/>
        <rdfs:range rdf:resource="https://w3id.org/cerif2/Resource"/>
        <rdfs:comment xml:lang="en">A Resource Request specifies the [Resource](../entities/Resource.md) that is the subject of the request.</rdfs:comment>
    </owl:ObjectProperty>
    


    <!-- https://w3id.org/cerif2/Resource_Usage_Statement#details -->


    <owl:ObjectProperty rdf:about="https://w3id.org/cerif2/Resource_Usage_Statement#details">
        <rdfs:domain rdf:resource="https://w3id.org/cerif2/Resource_Usage_Statement"/>
        <rdfs:range rdf:resource="https://w3id.org/cerif2/Contribution_Statement"/>
        <rdfs:comment xml:lang="en">A Resource Usage Statement can detail any number of [Contribution Statements](../entities/Contribution_Statement.md).</rdfs:comment>
    </owl:ObjectProperty>
    


    <!-- https://w3id.org/cerif2/Resource_Usage_Statement#uses -->


    <owl:ObjectProperty rdf:about="https://w3id.org/cerif2/Resource_Usage_Statement#uses">
        <rdfs:domain rdf:resource="https://w3id.org/cerif2/Resource_Usage_Statement"/>
        <rdfs:range rdf:resource="https://w3id.org/cerif2/Resource"/>
        <rdfs:comment xml:lang="en">A Resource Usage Statement specifies the [Resource](../entities/Resource.md) that is being used.</rdfs:comment>
    </owl:ObjectProperty>
    


    <!-- https://w3id.org/cerif2/Visiting_Address#physicalAddress -->


    <owl:ObjectProperty rdf:about="https://w3id.org/cerif2/Visiting_Address#physicalAddress">
        <rdfs:domain rdf:resource="https://w3id.org/cerif2/Visiting_Address"/>
        <rdfs:range rdf:resource="https://w3id.org/cerif2/Physical_Address"/>
    </owl:ObjectProperty>
    


    <!-- 
    ///////////////////////////////////////////////////////////////////////////////////////
    //
    // Data properties
    //
    ///////////////////////////////////////////////////////////////////////////////////////
     -->


    


    <!-- https://w3id.org/cerif2/Acknowledgement_Statement#statement -->


    <owl:DatatypeProperty rdf:about="https://w3id.org/cerif2/Acknowledgement_Statement#statement">
        <rdfs:domain rdf:resource="https://w3id.org/cerif2/Acknowledgement_Statement"/>
        <rdfs:range rdf:resource="https://w3id.org/cerif2/Multilingual_String"/>
    </owl:DatatypeProperty>
    


    <!-- https://w3id.org/cerif2/Affiliation_Statement#contacts -->


    <owl:DatatypeProperty rdf:about="https://w3id.org/cerif2/Affiliation_Statement#contacts">
        <rdfs:domain rdf:resource="https://w3id.org/cerif2/Affiliation_Statement"/>
        <rdfs:range rdf:resource="https://w3id.org/cerif2/Contact_Information"/>
    </owl:DatatypeProperty>
    


    <!-- https://w3id.org/cerif2/Affiliation_Statement#displayAffiliation -->


    <owl:DatatypeProperty rdf:about="https://w3id.org/cerif2/Affiliation_Statement#displayAffiliation">
        <rdfs:domain rdf:resource="https://w3id.org/cerif2/Affiliation_Statement"/>
        <rdfs:range rdf:resource="https://w3id.org/cerif2/Multilingual_String"/>
        <rdfs:label>the raw form of the affiliation as found e.g. in scholarly publications; more structured statements make use of the *institution* and/or *organisation unit* relationships below</rdfs:label>
    </owl:DatatypeProperty>
    


    <!-- https://w3id.org/cerif2/Affiliation_Statement#displayPersonName -->


    <owl:DatatypeProperty rdf:about="https://w3id.org/cerif2/Affiliation_Statement#displayPersonName">
        <rdfs:domain rdf:resource="https://w3id.org/cerif2/Affiliation_Statement"/>
        <rdfs:range rdf:resource="https://w3id.org/cerif2/Multilingual_String"/>
        <rdfs:label>the raw form of the name of the person as found e.g. in scholarly publications; more structured statements make use of the *person* relationship below</rdfs:label>
    </owl:DatatypeProperty>
    


    <!-- https://w3id.org/cerif2/Agent#contacts -->


    <owl:DatatypeProperty rdf:about="https://w3id.org/cerif2/Agent#contacts">
        <rdfs:domain rdf:resource="https://w3id.org/cerif2/Agent"/>
        <rdfs:range rdf:resource="https://w3id.org/cerif2/Contact_Information"/>
    </owl:DatatypeProperty>
    


    <!-- https://w3id.org/cerif2/Agent#keywords -->


    <owl:DatatypeProperty rdf:about="https://w3id.org/cerif2/Agent#keywords">
        <rdfs:domain rdf:resource="https://w3id.org/cerif2/Agent"/>
        <rdfs:range rdf:resource="https://w3id.org/cerif2/Multilingual_String"/>
    </owl:DatatypeProperty>
    


    <!-- https://w3id.org/cerif2/Call_for_Applications#deadline -->


    <owl:DatatypeProperty rdf:about="https://w3id.org/cerif2/Call_for_Applications#deadline">
        <rdfs:domain rdf:resource="https://w3id.org/cerif2/Call_for_Applications"/>
        <rdfs:range rdf:resource="https://w3id.org/cerif2/Date"/>
        <rdfs:label>until when applications can be submitted</rdfs:label>
    </owl:DatatypeProperty>
    


    <!-- https://w3id.org/cerif2/Contents_Location#number -->


    <owl:DatatypeProperty rdf:about="https://w3id.org/cerif2/Contents_Location#number">
        <rdfs:domain rdf:resource="https://w3id.org/cerif2/Contents_Location"/>
        <rdfs:range rdf:resource="https://w3id.org/cerif2/String"/>
    </owl:DatatypeProperty>
    


    <!-- https://w3id.org/cerif2/Contribution_Statement#statement -->


    <owl:DatatypeProperty rdf:about="https://w3id.org/cerif2/Contribution_Statement#statement">
        <rdfs:domain rdf:resource="https://w3id.org/cerif2/Contribution_Statement"/>
        <rdfs:range rdf:resource="https://w3id.org/cerif2/Multilingual_String"/>
    </owl:DatatypeProperty>
    


    <!-- https://w3id.org/cerif2/Country#iso3166Alpha2Code -->


    <owl:DatatypeProperty rdf:about="https://w3id.org/cerif2/Country#iso3166Alpha2Code">
        <rdfs:domain rdf:resource="https://w3id.org/cerif2/Country"/>
        <rdfs:range rdf:resource="https://w3id.org/cerif2/ISO_3166_Alpha2_Code"/>
        <rdfs:label> this should be the preferred way of referencing a country</rdfs:label>
    </owl:DatatypeProperty>
    


    <!-- https://w3id.org/cerif2/Country#name -->


    <owl:DatatypeProperty rdf:about="https://w3id.org/cerif2/Country#name">
        <rdfs:domain rdf:resource="https://w3id.org/cerif2/Country"/>
        <rdfs:range rdf:resource="https://w3id.org/cerif2/Multilingual_String"/>
    </owl:DatatypeProperty>
    


    <!-- https://w3id.org/cerif2/DOI_Identifier#doiId -->


    <owl:DatatypeProperty rdf:about="https://w3id.org/cerif2/DOI_Identifier#doiId">
        <rdfs:domain rdf:resource="https://w3id.org/cerif2/DOI_Identifier"/>
        <rdfs:range rdf:resource="https://w3id.org/cerif2/DOI_ID"/>
    </owl:DatatypeProperty>
    


    <!-- https://w3id.org/cerif2/Date_Range#endDate -->


    <owl:DatatypeProperty rdf:about="https://w3id.org/cerif2/Date_Range#endDate">
        <rdfs:domain rdf:resource="https://w3id.org/cerif2/Date_Range"/>
        <rdfs:range rdf:resource="https://w3id.org/cerif2/Date"/>
    </owl:DatatypeProperty>
    


    <!-- https://w3id.org/cerif2/Date_Range#endDateInclusive -->


    <owl:DatatypeProperty rdf:about="https://w3id.org/cerif2/Date_Range#endDateInclusive">
        <rdfs:domain rdf:resource="https://w3id.org/cerif2/Date_Range"/>
        <rdfs:range rdf:resource="https://w3id.org/cerif2/Boolean"/>
    </owl:DatatypeProperty>
    


    <!-- https://w3id.org/cerif2/Date_Range#startDate -->


    <owl:DatatypeProperty rdf:about="https://w3id.org/cerif2/Date_Range#startDate">
        <rdfs:domain rdf:resource="https://w3id.org/cerif2/Date_Range"/>
        <rdfs:range rdf:resource="https://w3id.org/cerif2/Date"/>
    </owl:DatatypeProperty>
    


    <!-- https://w3id.org/cerif2/Date_Range#startDateInclusive -->


    <owl:DatatypeProperty rdf:about="https://w3id.org/cerif2/Date_Range#startDateInclusive">
        <rdfs:domain rdf:resource="https://w3id.org/cerif2/Date_Range"/>
        <rdfs:range rdf:resource="https://w3id.org/cerif2/Boolean"/>
    </owl:DatatypeProperty>
    


    <!-- https://w3id.org/cerif2/Decision#date -->


    <owl:DatatypeProperty rdf:about="https://w3id.org/cerif2/Decision#date">
        <rdfs:domain rdf:resource="https://w3id.org/cerif2/Decision"/>
        <rdfs:range rdf:resource="https://w3id.org/cerif2/Date"/>
    </owl:DatatypeProperty>
    


    <!-- https://w3id.org/cerif2/Document#title -->


    <owl:DatatypeProperty rdf:about="https://w3id.org/cerif2/Document#title">
        <rdfs:domain rdf:resource="https://w3id.org/cerif2/Document"/>
        <rdfs:range rdf:resource="https://w3id.org/cerif2/Multilingual_String"/>
    </owl:DatatypeProperty>
    


    <!-- https://w3id.org/cerif2/Document_Publication#publicationDate -->


    <owl:DatatypeProperty rdf:about="https://w3id.org/cerif2/Document_Publication#publicationDate">
        <rdfs:domain rdf:resource="https://w3id.org/cerif2/Document_Publication"/>
        <rdfs:range rdf:resource="https://w3id.org/cerif2/Date"/>
    </owl:DatatypeProperty>
    


    <!-- https://w3id.org/cerif2/Education#completed -->


    <owl:DatatypeProperty rdf:about="https://w3id.org/cerif2/Education#completed">
        <rdfs:domain rdf:resource="https://w3id.org/cerif2/Education"/>
        <rdfs:range rdf:resource="https://w3id.org/cerif2/Boolean"/>
    </owl:DatatypeProperty>
    


    <!-- https://w3id.org/cerif2/Electronic_Address#uri -->


    <owl:DatatypeProperty rdf:about="https://w3id.org/cerif2/Electronic_Address#uri">
        <rdfs:domain rdf:resource="https://w3id.org/cerif2/Electronic_Address"/>
        <rdfs:range rdf:resource="https://w3id.org/cerif2/URI"/>
    </owl:DatatypeProperty>
    


    <!-- https://w3id.org/cerif2/Evaluation_Outcome#conslusions -->


    <owl:DatatypeProperty rdf:about="https://w3id.org/cerif2/Evaluation_Outcome#conslusions">
        <rdfs:domain rdf:resource="https://w3id.org/cerif2/Evaluation_Outcome"/>
        <rdfs:range rdf:resource="https://w3id.org/cerif2/Multilingual_String"/>
    </owl:DatatypeProperty>
    


    <!-- https://w3id.org/cerif2/Event#acronym -->


    <owl:DatatypeProperty rdf:about="https://w3id.org/cerif2/Event#acronym">
        <rdfs:domain rdf:resource="https://w3id.org/cerif2/Event"/>
        <rdfs:range rdf:resource="https://w3id.org/cerif2/Multilingual_String"/>
    </owl:DatatypeProperty>
    


    <!-- https://w3id.org/cerif2/Event#contacts -->


    <owl:DatatypeProperty rdf:about="https://w3id.org/cerif2/Event#contacts">
        <rdfs:domain rdf:resource="https://w3id.org/cerif2/Event"/>
        <rdfs:range rdf:resource="https://w3id.org/cerif2/Contact_Information"/>
    </owl:DatatypeProperty>
    


    <!-- https://w3id.org/cerif2/Event#description -->


    <owl:DatatypeProperty rdf:about="https://w3id.org/cerif2/Event#description">
        <rdfs:domain rdf:resource="https://w3id.org/cerif2/Event"/>
        <rdfs:range rdf:resource="https://w3id.org/cerif2/Multilingual_String"/>
    </owl:DatatypeProperty>
    


    <!-- https://w3id.org/cerif2/Event#ordinalNumber -->


    <owl:DatatypeProperty rdf:about="https://w3id.org/cerif2/Event#ordinalNumber">
        <rdfs:domain rdf:resource="https://w3id.org/cerif2/Event"/>
        <rdfs:range rdf:resource="https://w3id.org/cerif2/Decimal"/>
    </owl:DatatypeProperty>
    


    <!-- https://w3id.org/cerif2/Event#title -->


    <owl:DatatypeProperty rdf:about="https://w3id.org/cerif2/Event#title">
        <rdfs:domain rdf:resource="https://w3id.org/cerif2/Event"/>
        <rdfs:range rdf:resource="https://w3id.org/cerif2/Multilingual_String"/>
    </owl:DatatypeProperty>
    


    <!-- https://w3id.org/cerif2/Event_Series#acronym -->


    <owl:DatatypeProperty rdf:about="https://w3id.org/cerif2/Event_Series#acronym">
        <rdfs:domain rdf:resource="https://w3id.org/cerif2/Event_Series"/>
        <rdfs:range rdf:resource="https://w3id.org/cerif2/Multilingual_String"/>
    </owl:DatatypeProperty>
    


    <!-- https://w3id.org/cerif2/Event_Series#contacts -->


    <owl:DatatypeProperty rdf:about="https://w3id.org/cerif2/Event_Series#contacts">
        <rdfs:domain rdf:resource="https://w3id.org/cerif2/Event_Series"/>
        <rdfs:range rdf:resource="https://w3id.org/cerif2/Contact_Information"/>
    </owl:DatatypeProperty>
    


    <!-- https://w3id.org/cerif2/Event_Series#description -->


    <owl:DatatypeProperty rdf:about="https://w3id.org/cerif2/Event_Series#description">
        <rdfs:domain rdf:resource="https://w3id.org/cerif2/Event_Series"/>
        <rdfs:range rdf:resource="https://w3id.org/cerif2/Multilingual_String"/>
    </owl:DatatypeProperty>
    


    <!-- https://w3id.org/cerif2/Event_Series#recurrencePeriod -->


    <owl:DatatypeProperty rdf:about="https://w3id.org/cerif2/Event_Series#recurrencePeriod">
        <rdfs:domain rdf:resource="https://w3id.org/cerif2/Event_Series"/>
        <rdfs:range rdf:resource="https://w3id.org/cerif2/Decimal"/>
    </owl:DatatypeProperty>
    


    <!-- https://w3id.org/cerif2/Event_Series#recurrenceUnit -->


    <owl:DatatypeProperty rdf:about="https://w3id.org/cerif2/Event_Series#recurrenceUnit">
        <rdfs:domain rdf:resource="https://w3id.org/cerif2/Event_Series"/>
        <rdfs:range rdf:resource="https://w3id.org/cerif2/Multilingual_String"/>
    </owl:DatatypeProperty>
    


    <!-- https://w3id.org/cerif2/Event_Series#title -->


    <owl:DatatypeProperty rdf:about="https://w3id.org/cerif2/Event_Series#title">
        <rdfs:domain rdf:resource="https://w3id.org/cerif2/Event_Series"/>
        <rdfs:range rdf:resource="https://w3id.org/cerif2/Multilingual_String"/>
    </owl:DatatypeProperty>
    


    <!-- https://w3id.org/cerif2/Expertise_and_Skills#description -->


    <owl:DatatypeProperty rdf:about="https://w3id.org/cerif2/Expertise_and_Skills#description">
        <rdfs:domain rdf:resource="https://w3id.org/cerif2/Expertise_and_Skills"/>
        <rdfs:range rdf:resource="https://w3id.org/cerif2/Multilingual_String"/>
    </owl:DatatypeProperty>
    


    <!-- https://w3id.org/cerif2/Expertise_and_Skills#label -->


    <owl:DatatypeProperty rdf:about="https://w3id.org/cerif2/Expertise_and_Skills#label">
        <rdfs:domain rdf:resource="https://w3id.org/cerif2/Expertise_and_Skills"/>
        <rdfs:range rdf:resource="https://w3id.org/cerif2/Multilingual_String"/>
    </owl:DatatypeProperty>
    


    <!-- https://w3id.org/cerif2/Expertise_and_Time_and_Effort#amountOfTimeInPersonHours -->


    <owl:DatatypeProperty rdf:about="https://w3id.org/cerif2/Expertise_and_Time_and_Effort#amountOfTimeInPersonHours">
        <rdfs:domain rdf:resource="https://w3id.org/cerif2/Expertise_and_Time_and_Effort"/>
        <rdfs:range rdf:resource="https://w3id.org/cerif2/Decimal"/>
    </owl:DatatypeProperty>
    


    <!-- https://w3id.org/cerif2/FundRef_Identifier#fundrefId -->


    <owl:DatatypeProperty rdf:about="https://w3id.org/cerif2/FundRef_Identifier#fundrefId">
        <rdfs:domain rdf:resource="https://w3id.org/cerif2/FundRef_Identifier"/>
        <rdfs:range rdf:resource="https://w3id.org/cerif2/FundRef_ID"/>
    </owl:DatatypeProperty>
    


    <!-- https://w3id.org/cerif2/Group_or_Organisation_Unit#acronym -->


    <owl:DatatypeProperty rdf:about="https://w3id.org/cerif2/Group_or_Organisation_Unit#acronym">
        <rdfs:domain rdf:resource="https://w3id.org/cerif2/Group_or_Organisation_Unit"/>
        <rdfs:range rdf:resource="https://w3id.org/cerif2/Multilingual_String"/>
    </owl:DatatypeProperty>
    


    <!-- https://w3id.org/cerif2/Group_or_Organisation_Unit#description -->


    <owl:DatatypeProperty rdf:about="https://w3id.org/cerif2/Group_or_Organisation_Unit#description">
        <rdfs:domain rdf:resource="https://w3id.org/cerif2/Group_or_Organisation_Unit"/>
        <rdfs:range rdf:resource="https://w3id.org/cerif2/Multilingual_String"/>
    </owl:DatatypeProperty>
    


    <!-- https://w3id.org/cerif2/Group_or_Organisation_Unit#name -->


    <owl:DatatypeProperty rdf:about="https://w3id.org/cerif2/Group_or_Organisation_Unit#name">
        <rdfs:domain rdf:resource="https://w3id.org/cerif2/Group_or_Organisation_Unit"/>
        <rdfs:range rdf:resource="https://w3id.org/cerif2/Multilingual_String"/>
    </owl:DatatypeProperty>
    


    <!-- https://w3id.org/cerif2/ISNI_Identifier#isniId -->


    <owl:DatatypeProperty rdf:about="https://w3id.org/cerif2/ISNI_Identifier#isniId">
        <rdfs:domain rdf:resource="https://w3id.org/cerif2/ISNI_Identifier"/>
        <rdfs:range rdf:resource="https://w3id.org/cerif2/ISNI_ID"/>
    </owl:DatatypeProperty>
    


    <!-- https://w3id.org/cerif2/Infrastructure#acronym -->


    <owl:DatatypeProperty rdf:about="https://w3id.org/cerif2/Infrastructure#acronym">
        <rdfs:domain rdf:resource="https://w3id.org/cerif2/Infrastructure"/>
        <rdfs:range rdf:resource="https://w3id.org/cerif2/Multilingual_String"/>
    </owl:DatatypeProperty>
    


    <!-- https://w3id.org/cerif2/Infrastructure#title -->


    <owl:DatatypeProperty rdf:about="https://w3id.org/cerif2/Infrastructure#title">
        <rdfs:domain rdf:resource="https://w3id.org/cerif2/Infrastructure"/>
        <rdfs:range rdf:resource="https://w3id.org/cerif2/Multilingual_String"/>
    </owl:DatatypeProperty>
    


    <!-- https://w3id.org/cerif2/Infrastructure#url -->


    <owl:DatatypeProperty rdf:about="https://w3id.org/cerif2/Infrastructure#url">
        <rdfs:domain rdf:resource="https://w3id.org/cerif2/Infrastructure"/>
        <rdfs:range rdf:resource="https://w3id.org/cerif2/Website_Address"/>
    </owl:DatatypeProperty>
    


    <!-- https://w3id.org/cerif2/Involvement#description -->


    <owl:DatatypeProperty rdf:about="https://w3id.org/cerif2/Involvement#description">
        <rdfs:domain rdf:resource="https://w3id.org/cerif2/Involvement"/>
        <rdfs:range rdf:resource="https://w3id.org/cerif2/Multilingual_String"/>
    </owl:DatatypeProperty>
    


    <!-- https://w3id.org/cerif2/Language#iso6391Code -->


    <owl:DatatypeProperty rdf:about="https://w3id.org/cerif2/Language#iso6391Code">
        <rdfs:domain rdf:resource="https://w3id.org/cerif2/Language"/>
        <rdfs:range rdf:resource="https://w3id.org/cerif2/ISO_639_1_Alpha2_Code"/>
    </owl:DatatypeProperty>
    


    <!-- https://w3id.org/cerif2/Language#iso6392bCode -->


    <owl:DatatypeProperty rdf:about="https://w3id.org/cerif2/Language#iso6392bCode">
        <rdfs:domain rdf:resource="https://w3id.org/cerif2/Language"/>
        <rdfs:range rdf:resource="https://w3id.org/cerif2/ISO_639_2B_Alpha3_Code"/>
    </owl:DatatypeProperty>
    


    <!-- https://w3id.org/cerif2/Language#iso6392tCode -->


    <owl:DatatypeProperty rdf:about="https://w3id.org/cerif2/Language#iso6392tCode">
        <rdfs:domain rdf:resource="https://w3id.org/cerif2/Language"/>
        <rdfs:range rdf:resource="https://w3id.org/cerif2/ISO_639_2T_Alpha3_Code"/>
    </owl:DatatypeProperty>
    


    <!-- https://w3id.org/cerif2/Language#name -->


    <owl:DatatypeProperty rdf:about="https://w3id.org/cerif2/Language#name">
        <rdfs:domain rdf:resource="https://w3id.org/cerif2/Language"/>
        <rdfs:range rdf:resource="https://w3id.org/cerif2/Multilingual_String"/>
    </owl:DatatypeProperty>
    


    <!-- https://w3id.org/cerif2/Local_Agent_Identifier#localId -->


    <owl:DatatypeProperty rdf:about="https://w3id.org/cerif2/Local_Agent_Identifier#localId">
        <rdfs:domain rdf:resource="https://w3id.org/cerif2/Local_Agent_Identifier"/>
        <rdfs:range rdf:resource="https://w3id.org/cerif2/Local_Agent_ID"/>
    </owl:DatatypeProperty>
    


    <!-- https://w3id.org/cerif2/Local_Resource_Identifier#localId -->


    <owl:DatatypeProperty rdf:about="https://w3id.org/cerif2/Local_Resource_Identifier#localId">
        <rdfs:domain rdf:resource="https://w3id.org/cerif2/Local_Resource_Identifier"/>
        <rdfs:range rdf:resource="https://w3id.org/cerif2/Local_Resource_ID"/>
    </owl:DatatypeProperty>
    


    <!-- https://w3id.org/cerif2/Monetary_Amount#amount -->


    <owl:DatatypeProperty rdf:about="https://w3id.org/cerif2/Monetary_Amount#amount">
        <rdfs:domain rdf:resource="https://w3id.org/cerif2/Monetary_Amount"/>
        <rdfs:range rdf:resource="https://w3id.org/cerif2/Decimal"/>
        <rdfs:label> mandatory</rdfs:label>
    </owl:DatatypeProperty>
    


    <!-- https://w3id.org/cerif2/Monetary_Amount#currencyCode -->


    <owl:DatatypeProperty rdf:about="https://w3id.org/cerif2/Monetary_Amount#currencyCode">
        <rdfs:domain rdf:resource="https://w3id.org/cerif2/Monetary_Amount"/>
        <rdfs:range rdf:resource="https://w3id.org/cerif2/ISO_4217_Alpha_Code"/>
        <rdfs:label> mandatory</rdfs:label>
    </owl:DatatypeProperty>
    


    <!-- https://w3id.org/cerif2/ORCID_Identifier#orcidId -->


    <owl:DatatypeProperty rdf:about="https://w3id.org/cerif2/ORCID_Identifier#orcidId">
        <rdfs:domain rdf:resource="https://w3id.org/cerif2/ORCID_Identifier"/>
        <rdfs:range rdf:resource="https://w3id.org/cerif2/ORCID_iD"/>
    </owl:DatatypeProperty>
    


    <!-- https://w3id.org/cerif2/Page_Based_Contents_Location#endPage -->


    <owl:DatatypeProperty rdf:about="https://w3id.org/cerif2/Page_Based_Contents_Location#endPage">
        <rdfs:domain rdf:resource="https://w3id.org/cerif2/Page_Based_Contents_Location"/>
        <rdfs:range rdf:resource="https://w3id.org/cerif2/String"/>
    </owl:DatatypeProperty>
    


    <!-- https://w3id.org/cerif2/Page_Based_Contents_Location#startPage -->


    <owl:DatatypeProperty rdf:about="https://w3id.org/cerif2/Page_Based_Contents_Location#startPage">
        <rdfs:domain rdf:resource="https://w3id.org/cerif2/Page_Based_Contents_Location"/>
        <rdfs:range rdf:resource="https://w3id.org/cerif2/String"/>
    </owl:DatatypeProperty>
    


    <!-- https://w3id.org/cerif2/Person_Name#displayName -->


    <owl:DatatypeProperty rdf:about="https://w3id.org/cerif2/Person_Name#displayName">
        <rdfs:domain rdf:resource="https://w3id.org/cerif2/Person_Name"/>
        <rdfs:range rdf:resource="https://w3id.org/cerif2/Multilingual_String"/>
    </owl:DatatypeProperty>
    


    <!-- https://w3id.org/cerif2/Person_Name#familyNames -->


    <owl:DatatypeProperty rdf:about="https://w3id.org/cerif2/Person_Name#familyNames">
        <rdfs:domain rdf:resource="https://w3id.org/cerif2/Person_Name"/>
        <rdfs:range rdf:resource="https://w3id.org/cerif2/Multilingual_String"/>
    </owl:DatatypeProperty>
    


    <!-- https://w3id.org/cerif2/Person_Name#firstNames -->


    <owl:DatatypeProperty rdf:about="https://w3id.org/cerif2/Person_Name#firstNames">
        <rdfs:domain rdf:resource="https://w3id.org/cerif2/Person_Name"/>
        <rdfs:range rdf:resource="https://w3id.org/cerif2/Multilingual_String"/>
    </owl:DatatypeProperty>
    


    <!-- https://w3id.org/cerif2/Person_Name#otherNames -->


    <owl:DatatypeProperty rdf:about="https://w3id.org/cerif2/Person_Name#otherNames">
        <rdfs:domain rdf:resource="https://w3id.org/cerif2/Person_Name"/>
        <rdfs:range rdf:resource="https://w3id.org/cerif2/Multilingual_String"/>
    </owl:DatatypeProperty>
    


    <!-- https://w3id.org/cerif2/Position#code -->


    <owl:DatatypeProperty rdf:about="https://w3id.org/cerif2/Position#code">
        <rdfs:domain rdf:resource="https://w3id.org/cerif2/Position"/>
        <rdfs:range rdf:resource="https://w3id.org/cerif2/String"/>
    </owl:DatatypeProperty>
    


    <!-- https://w3id.org/cerif2/Position#title -->


    <owl:DatatypeProperty rdf:about="https://w3id.org/cerif2/Position#title">
        <rdfs:domain rdf:resource="https://w3id.org/cerif2/Position"/>
        <rdfs:range rdf:resource="https://w3id.org/cerif2/Multilingual_String"/>
    </owl:DatatypeProperty>
    


    <!-- https://w3id.org/cerif2/Prize#name -->


    <owl:DatatypeProperty rdf:about="https://w3id.org/cerif2/Prize#name">
        <rdfs:domain rdf:resource="https://w3id.org/cerif2/Prize"/>
        <rdfs:range rdf:resource="https://w3id.org/cerif2/Multilingual_String"/>
    </owl:DatatypeProperty>
    


    <!-- https://w3id.org/cerif2/Project#acronym -->


    <owl:DatatypeProperty rdf:about="https://w3id.org/cerif2/Project#acronym">
        <rdfs:domain rdf:resource="https://w3id.org/cerif2/Project"/>
        <rdfs:range rdf:resource="https://w3id.org/cerif2/Multilingual_String"/>
    </owl:DatatypeProperty>
    


    <!-- https://w3id.org/cerif2/Project#name -->


    <owl:DatatypeProperty rdf:about="https://w3id.org/cerif2/Project#name">
        <rdfs:domain rdf:resource="https://w3id.org/cerif2/Project"/>
        <rdfs:range rdf:resource="https://w3id.org/cerif2/Multilingual_String"/>
    </owl:DatatypeProperty>
    


    <!-- https://w3id.org/cerif2/Publication_Channel#acronym -->


    <owl:DatatypeProperty rdf:about="https://w3id.org/cerif2/Publication_Channel#acronym">
        <rdfs:domain rdf:resource="https://w3id.org/cerif2/Publication_Channel"/>
        <rdfs:range rdf:resource="https://w3id.org/cerif2/Multilingual_String"/>
    </owl:DatatypeProperty>
    


    <!-- https://w3id.org/cerif2/Publication_Channel#title -->


    <owl:DatatypeProperty rdf:about="https://w3id.org/cerif2/Publication_Channel#title">
        <rdfs:domain rdf:resource="https://w3id.org/cerif2/Publication_Channel"/>
        <rdfs:range rdf:resource="https://w3id.org/cerif2/Multilingual_String"/>
    </owl:DatatypeProperty>
    


    <!-- https://w3id.org/cerif2/ROR_Identifier#rorId -->


    <owl:DatatypeProperty rdf:about="https://w3id.org/cerif2/ROR_Identifier#rorId">
        <rdfs:domain rdf:resource="https://w3id.org/cerif2/ROR_Identifier"/>
        <rdfs:range rdf:resource="https://w3id.org/cerif2/ROR_ID"/>
    </owl:DatatypeProperty>
    


    <!-- https://w3id.org/cerif2/Resource_Request#requestDate -->


    <owl:DatatypeProperty rdf:about="https://w3id.org/cerif2/Resource_Request#requestDate">
        <rdfs:domain rdf:resource="https://w3id.org/cerif2/Resource_Request"/>
        <rdfs:range rdf:resource="https://w3id.org/cerif2/Date"/>
    </owl:DatatypeProperty>
    


    <!-- https://w3id.org/cerif2/Resource_Usage_Statement#statement -->


    <owl:DatatypeProperty rdf:about="https://w3id.org/cerif2/Resource_Usage_Statement#statement">
        <rdfs:domain rdf:resource="https://w3id.org/cerif2/Resource_Usage_Statement"/>
        <rdfs:range rdf:resource="https://w3id.org/cerif2/Multilingual_String"/>
    </owl:DatatypeProperty>
    


    <!-- https://w3id.org/cerif2/Script#name -->


    <owl:DatatypeProperty rdf:about="https://w3id.org/cerif2/Script#name">
        <rdfs:domain rdf:resource="https://w3id.org/cerif2/Script"/>
        <rdfs:range rdf:resource="https://w3id.org/cerif2/Multilingual_String"/>
    </owl:DatatypeProperty>
    


    <!-- https://w3id.org/cerif2/Script#scriptCode -->


    <owl:DatatypeProperty rdf:about="https://w3id.org/cerif2/Script#scriptCode">
        <rdfs:domain rdf:resource="https://w3id.org/cerif2/Script"/>
        <rdfs:range rdf:resource="https://w3id.org/cerif2/ISO_15924_Alpha4_Code"/>
    </owl:DatatypeProperty>
    


    <!-- https://w3id.org/cerif2/Simple_Physical_Address#address -->


    <owl:DatatypeProperty rdf:about="https://w3id.org/cerif2/Simple_Physical_Address#address">
        <rdfs:domain rdf:resource="https://w3id.org/cerif2/Simple_Physical_Address"/>
        <rdfs:range rdf:resource="https://w3id.org/cerif2/Multilingual_String"/>
    </owl:DatatypeProperty>
    


    <!-- https://w3id.org/cerif2/Structured_Physical_Address#city -->


    <owl:DatatypeProperty rdf:about="https://w3id.org/cerif2/Structured_Physical_Address#city">
        <rdfs:domain rdf:resource="https://w3id.org/cerif2/Structured_Physical_Address"/>
        <rdfs:range rdf:resource="https://w3id.org/cerif2/Multilingual_String"/>
    </owl:DatatypeProperty>
    


    <!-- https://w3id.org/cerif2/Structured_Physical_Address#stateOrProvince -->


    <owl:DatatypeProperty rdf:about="https://w3id.org/cerif2/Structured_Physical_Address#stateOrProvince">
        <rdfs:domain rdf:resource="https://w3id.org/cerif2/Structured_Physical_Address"/>
        <rdfs:range rdf:resource="https://w3id.org/cerif2/Multilingual_String"/>
    </owl:DatatypeProperty>
    


    <!-- https://w3id.org/cerif2/Structured_Physical_Address#street -->


    <owl:DatatypeProperty rdf:about="https://w3id.org/cerif2/Structured_Physical_Address#street">
        <rdfs:domain rdf:resource="https://w3id.org/cerif2/Structured_Physical_Address"/>
        <rdfs:range rdf:resource="https://w3id.org/cerif2/Multilingual_String"/>
    </owl:DatatypeProperty>
    


    <!-- https://w3id.org/cerif2/Structured_Physical_Address#zipCode -->


    <owl:DatatypeProperty rdf:about="https://w3id.org/cerif2/Structured_Physical_Address#zipCode">
        <rdfs:domain rdf:resource="https://w3id.org/cerif2/Structured_Physical_Address"/>
        <rdfs:range rdf:resource="https://w3id.org/cerif2/Multilingual_String"/>
    </owl:DatatypeProperty>
    


    <!-- https://w3id.org/cerif2/Time_Based_Contents_Location#endTime -->


    <owl:DatatypeProperty rdf:about="https://w3id.org/cerif2/Time_Based_Contents_Location#endTime">
        <rdfs:domain rdf:resource="https://w3id.org/cerif2/Time_Based_Contents_Location"/>
        <rdfs:range rdf:resource="https://w3id.org/cerif2/Time"/>
    </owl:DatatypeProperty>
    


    <!-- https://w3id.org/cerif2/Time_Based_Contents_Location#startTime -->


    <owl:DatatypeProperty rdf:about="https://w3id.org/cerif2/Time_Based_Contents_Location#startTime">
        <rdfs:domain rdf:resource="https://w3id.org/cerif2/Time_Based_Contents_Location"/>
        <rdfs:range rdf:resource="https://w3id.org/cerif2/Time"/>
    </owl:DatatypeProperty>
    


    <!-- https://w3id.org/cerif2/Wikidata_Agent_Identifier#wikidataId -->


    <owl:DatatypeProperty rdf:about="https://w3id.org/cerif2/Wikidata_Agent_Identifier#wikidataId">
        <rdfs:domain rdf:resource="https://w3id.org/cerif2/Wikidata_Agent_Identifier"/>
        <rdfs:range rdf:resource="https://w3id.org/cerif2/Wikidata_ID"/>
    </owl:DatatypeProperty>
    


    <!-- https://w3id.org/cerif2/Wikidata_Resource_Identifier#wikidataId -->


    <owl:DatatypeProperty rdf:about="https://w3id.org/cerif2/Wikidata_Resource_Identifier#wikidataId">
        <rdfs:domain rdf:resource="https://w3id.org/cerif2/Wikidata_Resource_Identifier"/>
        <rdfs:range rdf:resource="https://w3id.org/cerif2/Wikidata_ID"/>
    </owl:DatatypeProperty>
    


    <!-- 
    ///////////////////////////////////////////////////////////////////////////////////////
    //
    // Classes
    //
    ///////////////////////////////////////////////////////////////////////////////////////
     -->


    


    <!-- https://w3id.org/cerif2/Accessible_on_the_Web -->


    <owl:Class rdf:about="https://w3id.org/cerif2/Accessible_on_the_Web">
        <rdfs:comment xml:lang="en">Anything that can be accessed on the World Wide Web.</rdfs:comment>
        <rdfs:label xml:lang="en">Accessible on the Web</rdfs:label>
    </owl:Class>
    


    <!-- https://w3id.org/cerif2/Acknowledgement_Statement -->


    <owl:Class rdf:about="https://w3id.org/cerif2/Acknowledgement_Statement">
        <rdfs:comment xml:lang="en">Anything that testifies, demonstrates or acknowledges a [Contribution](../entities/Contribution.md).</rdfs:comment>
        <rdfs:label xml:lang="en">Acknowledgement Statement</rdfs:label>
    </owl:Class>
    


    <!-- https://w3id.org/cerif2/Activity -->


    <owl:Class rdf:about="https://w3id.org/cerif2/Activity">
        <rdfs:comment xml:lang="en">Anything an Agent does.</rdfs:comment>
        <rdfs:label xml:lang="en">Activity</rdfs:label>
    </owl:Class>
    


    <!-- https://w3id.org/cerif2/Affiliation_Statement -->


    <owl:Class rdf:about="https://w3id.org/cerif2/Affiliation_Statement">
        <rdfs:comment xml:lang="en">A statement of a connection between a [Person](../entities/Person.md) and an [Organisation Unit](../entities/Organisation_Unit.md).</rdfs:comment>
        <rdfs:label xml:lang="en">Affiliation Statement</rdfs:label>
    </owl:Class>
    


    <!-- https://w3id.org/cerif2/Agent -->


    <owl:Class rdf:about="https://w3id.org/cerif2/Agent">
        <rdfs:comment xml:lang="en">Anything that has the ability to perform activities.</rdfs:comment>
        <rdfs:label xml:lang="en">Agent</rdfs:label>
    </owl:Class>
    


    <!-- https://w3id.org/cerif2/Agent_Identifier -->


    <owl:Class rdf:about="https://w3id.org/cerif2/Agent_Identifier">
        <rdfs:comment xml:lang="en">An identifier that is assigned to an [Agent](../entities/Agent.md).</rdfs:comment>
        <rdfs:label xml:lang="en">Agent Identifier</rdfs:label>
    </owl:Class>
    


    <!-- https://w3id.org/cerif2/Application -->


    <owl:Class rdf:about="https://w3id.org/cerif2/Application">
        <rdfs:subClassOf rdf:resource="https://w3id.org/cerif2/Resource_Request"/>
        <rdfs:comment xml:lang="en">A formal request to be considered for a position or to be allowed to do or have something, submitted to an authority, institution, or organization.&lt;sup&gt;[1](#fn1)&lt;/sup&gt;</rdfs:comment>
        <rdfs:label xml:lang="en">Application</rdfs:label>
    </owl:Class>
    


    <!-- https://w3id.org/cerif2/Application_Review -->


    <owl:Class rdf:about="https://w3id.org/cerif2/Application_Review">
        <rdfs:subClassOf rdf:resource="https://w3id.org/cerif2/Contribution_to_Evaluation_Outcome"/>
        <rdfs:comment xml:lang="en">Any contribution to an [Evaluation Outcome](../entities/Evaluation_Outcome.md) of an [Application](../entities/Application.md) an [Agent](../entities/Agent.md) made by reviewing the Application.</rdfs:comment>
        <rdfs:label xml:lang="en">Application Review</rdfs:label>
    </owl:Class>
    


    <!-- https://w3id.org/cerif2/Audio_Contents -->


    <owl:Class rdf:about="https://w3id.org/cerif2/Audio_Contents">
        <rdfs:comment xml:lang="en">A resource primarily intended to be heard.&lt;sup&gt;[1](#fn1)&lt;/sup&gt;</rdfs:comment>
        <rdfs:label xml:lang="en">Audio Contents</rdfs:label>
    </owl:Class>
    


    <!-- https://w3id.org/cerif2/Call_for_Applications -->


    <owl:Class rdf:about="https://w3id.org/cerif2/Call_for_Applications">
        <rdfs:subClassOf rdf:resource="https://w3id.org/cerif2/Resource_Offer"/>
        <rdfs:comment xml:lang="en">A written or verbal request inviting someone to go somewhere or to do something,&lt;sup&gt;[1](#fn1)&lt;/sup&gt;
namely, submit an [Application](../entities/Application.md).</rdfs:comment>
        <rdfs:label xml:lang="en">Call for Applications</rdfs:label>
    </owl:Class>
    


    <!-- https://w3id.org/cerif2/Call_for_Funding_Applications -->


    <owl:Class rdf:about="https://w3id.org/cerif2/Call_for_Funding_Applications">
        <rdfs:subClassOf rdf:resource="https://w3id.org/cerif2/Call_for_Applications"/>
        <rdfs:comment xml:lang="en">A [Call for Applications](../entities/Call_for_Applications.md) that expects [Funding Applications](../entities/Funding_Application.md).</rdfs:comment>
        <rdfs:label xml:lang="en">Call for Funding Applications</rdfs:label>
    </owl:Class>
    


    <!-- https://w3id.org/cerif2/Condition -->


    <owl:Class rdf:about="https://w3id.org/cerif2/Condition">
        <rdfs:comment xml:lang="en">A condition that needs to be satisfied for a Resource Offer to be applicable.&lt;sup&gt;[1](#fn1)&lt;/sup&gt;</rdfs:comment>
        <rdfs:label xml:lang="en">Condition</rdfs:label>
    </owl:Class>
    


    <!-- https://w3id.org/cerif2/Contents_Location -->


    <owl:Class rdf:about="https://w3id.org/cerif2/Contents_Location">
        <rdfs:comment xml:lang="en">Location of contents of a [Document](../entities/Document.md).</rdfs:comment>
        <rdfs:label xml:lang="en">Contents Location</rdfs:label>
    </owl:Class>
    


    <!-- https://w3id.org/cerif2/Contribution -->


    <owl:Class rdf:about="https://w3id.org/cerif2/Contribution">
        <rdfs:subClassOf rdf:resource="https://w3id.org/cerif2/Activity"/>
        <rdfs:comment xml:lang="en">An activity that helps achieve a goal.</rdfs:comment>
        <rdfs:label xml:lang="en">Contribution</rdfs:label>
    </owl:Class>
    


    <!-- https://w3id.org/cerif2/Contribution_Statement -->


    <owl:Class rdf:about="https://w3id.org/cerif2/Contribution_Statement">
        <rdfs:comment xml:lang="en">An element of a [Contribution](../entities/Contribution.md). All such elements taken together describe the Contribution.</rdfs:comment>
        <rdfs:label xml:lang="en">Contribution Statement</rdfs:label>
    </owl:Class>
    


    <!-- https://w3id.org/cerif2/Contribution_to_Document -->


    <owl:Class rdf:about="https://w3id.org/cerif2/Contribution_to_Document">
        <rdfs:comment xml:lang="en">Any contribution an [Agent](../entities/Agent.md) made to a [Document](../entities/Document.md).</rdfs:comment>
        <rdfs:label xml:lang="en">Contribution to Document</rdfs:label>
    </owl:Class>
    


    <!-- https://w3id.org/cerif2/Contribution_to_Evaluation_Outcome -->


    <owl:Class rdf:about="https://w3id.org/cerif2/Contribution_to_Evaluation_Outcome">
        <rdfs:comment xml:lang="en">Any contribution an [Agent](../entities/Agent.md) made to an [Evaluation Outcome](../entities/Evaluation_Outcome.md).</rdfs:comment>
        <rdfs:label xml:lang="en">Contribution to Evaluation Outcome</rdfs:label>
    </owl:Class>
    


    <!-- https://w3id.org/cerif2/Contribution_to_Event -->


    <owl:Class rdf:about="https://w3id.org/cerif2/Contribution_to_Event">
        <rdfs:subClassOf rdf:resource="https://w3id.org/cerif2/Contribution"/>
        <rdfs:comment xml:lang="en">Any contribution an [Agent](../entities/Agent.md) made to an [Event](../entities/Event.md).</rdfs:comment>
        <rdfs:label xml:lang="en">Contribution to Event</rdfs:label>
    </owl:Class>
    


    <!-- https://w3id.org/cerif2/Contribution_to_Infrastructure -->


    <owl:Class rdf:about="https://w3id.org/cerif2/Contribution_to_Infrastructure">
        <rdfs:subClassOf rdf:resource="https://w3id.org/cerif2/Contribution"/>
        <rdfs:comment xml:lang="en">Any contribution an [Agent](../entities/Agent.md) made to an [Infrastructure](../entities/Infrastructure.md).</rdfs:comment>
        <rdfs:label xml:lang="en">Contribution to Infrastructure</rdfs:label>
    </owl:Class>
    


    <!-- https://w3id.org/cerif2/Contribution_to_Prize -->


    <owl:Class rdf:about="https://w3id.org/cerif2/Contribution_to_Prize">
        <rdfs:subClassOf rdf:resource="https://w3id.org/cerif2/Contribution"/>
        <rdfs:comment xml:lang="en">Any contribution an [Agent](../entities/Agent.md) made to a [Prize](../entities/Prize.md).</rdfs:comment>
        <rdfs:label xml:lang="en">Contribution to Prize</rdfs:label>
    </owl:Class>
    


    <!-- https://w3id.org/cerif2/Contribution_to_Prize_Award -->


    <owl:Class rdf:about="https://w3id.org/cerif2/Contribution_to_Prize_Award">
        <rdfs:subClassOf rdf:resource="https://w3id.org/cerif2/Contribution"/>
        <rdfs:comment xml:lang="en">Any contribution an [Agent](../entities/Agent.md) made to a [Prize Award](../entities/Prize_Award.md).</rdfs:comment>
        <rdfs:label xml:lang="en">Contribution to Prize Award</rdfs:label>
    </owl:Class>
    


    <!-- https://w3id.org/cerif2/Contribution_to_Project -->


    <owl:Class rdf:about="https://w3id.org/cerif2/Contribution_to_Project">
        <rdfs:comment xml:lang="en">Any contribution an [Agent](../entities/Agent.md) made to a [Project](../entities/Resource.md).</rdfs:comment>
        <rdfs:label xml:lang="en">Contribution to Project</rdfs:label>
    </owl:Class>
    


    <!-- https://w3id.org/cerif2/Country -->


    <owl:Class rdf:about="https://w3id.org/cerif2/Country">
        <rdfs:comment xml:lang="en">An area of land that has or used to have its own government and laws.&lt;sup&gt;[1](#fn1)&lt;/sup&gt;</rdfs:comment>
        <rdfs:label xml:lang="en">Country</rdfs:label>
    </owl:Class>
    


    <!-- https://w3id.org/cerif2/DOI_Identifier -->


    <owl:Class rdf:about="https://w3id.org/cerif2/DOI_Identifier">
        <rdfs:subClassOf rdf:resource="https://w3id.org/cerif2/Resource_Identifier"/>
        <rdfs:comment xml:lang="en">A DOI&lt;sup&gt;[1](#fn1)&lt;/sup&gt; identifier assigned to a [Document](../entities/Document.md).</rdfs:comment>
        <rdfs:label xml:lang="en">DOI Identifier</rdfs:label>
    </owl:Class>
    


    <!-- https://w3id.org/cerif2/Date_Range -->


    <owl:Class rdf:about="https://w3id.org/cerif2/Date_Range">
        <rdfs:comment xml:lang="en">A range of [Dates](../datatypes/Date.md).</rdfs:comment>
        <rdfs:label xml:lang="en">Date Range</rdfs:label>
    </owl:Class>
    


    <!-- https://w3id.org/cerif2/Decision -->


    <owl:Class rdf:about="https://w3id.org/cerif2/Decision">
        <rdfs:comment xml:lang="en">The conclusions from considering a [Resource Request](../entities/Resource_Request.md).</rdfs:comment>
        <rdfs:label xml:lang="en">Decision</rdfs:label>
    </owl:Class>
    


    <!-- https://w3id.org/cerif2/Document -->


    <owl:Class rdf:about="https://w3id.org/cerif2/Document">
        <rdfs:subClassOf rdf:resource="https://w3id.org/cerif2/Resource"/>
        <rdfs:comment xml:lang="en">A document is a bounded representation of a body of information designed with the capacity (and usually intent) to communicate. 
A document may manifest symbolic, diagrammatic or sensory-representational information.&lt;sup&gt;[1](#fn1)&lt;/sup&gt;</rdfs:comment>
        <rdfs:label xml:lang="en">Document</rdfs:label>
    </owl:Class>
    


    <!-- https://w3id.org/cerif2/Document_Publication -->


    <owl:Class rdf:about="https://w3id.org/cerif2/Document_Publication">
        <rdfs:comment xml:lang="en">The act of making information or stories available to people in a printed or electronic form.&lt;sup&gt;[1](#fn1)&lt;/sup&gt;</rdfs:comment>
        <rdfs:label xml:lang="en">Document Publication</rdfs:label>
    </owl:Class>
    


    <!-- https://w3id.org/cerif2/Downloadable -->


    <owl:Class rdf:about="https://w3id.org/cerif2/Downloadable">
        <rdfs:comment xml:lang="en">Anything that can be downloaded from the World Wide Web.</rdfs:comment>
        <rdfs:label xml:lang="en">Downloadable</rdfs:label>
    </owl:Class>
    


    <!-- https://w3id.org/cerif2/Education -->


    <owl:Class rdf:about="https://w3id.org/cerif2/Education">
        <rdfs:subClassOf rdf:resource="https://w3id.org/cerif2/Involvement"/>
        <rdfs:comment xml:lang="en">The process of (teaching or) learning, especially in a school or college, or the knowledge that you get from this.&lt;sup&gt;[1](#fn1)&lt;/sup&gt;</rdfs:comment>
        <rdfs:label xml:lang="en">Education</rdfs:label>
    </owl:Class>
    


    <!-- https://w3id.org/cerif2/Electronic_Address -->


    <owl:Class rdf:about="https://w3id.org/cerif2/Electronic_Address">
        <rdfs:subClassOf rdf:resource="https://w3id.org/cerif2/Contact_Information"/>
        <rdfs:comment xml:lang="en">An electronic address assigned to an [Agent](../entities/Organisation_Unit.md).</rdfs:comment>
        <rdfs:label xml:lang="en">Electronic Address</rdfs:label>
    </owl:Class>
    


    <!-- https://w3id.org/cerif2/Employment -->


    <owl:Class rdf:about="https://w3id.org/cerif2/Employment">
        <rdfs:subClassOf rdf:resource="https://w3id.org/cerif2/Involvement"/>
        <rdfs:comment xml:lang="en">Work that you are paid to do for a particular company or organization.&lt;sup&gt;[1](#fn1)&lt;/sup&gt;</rdfs:comment>
        <rdfs:label xml:lang="en">Employment</rdfs:label>
    </owl:Class>
    


    <!-- https://w3id.org/cerif2/Evaluation_Outcome -->


    <owl:Class rdf:about="https://w3id.org/cerif2/Evaluation_Outcome">
        <rdfs:comment xml:lang="en">The conclusions of an evaluation process.</rdfs:comment>
        <rdfs:label xml:lang="en">Decision</rdfs:label>
    </owl:Class>
    


    <!-- https://w3id.org/cerif2/Event -->


    <owl:Class rdf:about="https://w3id.org/cerif2/Event">
        <rdfs:comment xml:lang="en">A thing that happens, especially something important.&lt;sup&gt;[1](#fn1)&lt;/sup&gt;</rdfs:comment>
        <rdfs:label xml:lang="en">Event</rdfs:label>
    </owl:Class>
    


    <!-- https://w3id.org/cerif2/Event_Identifier -->


    <owl:Class rdf:about="https://w3id.org/cerif2/Event_Identifier">
        <rdfs:comment xml:lang="en">An identifier that is assigned to an [Event](../entities/Event.md).</rdfs:comment>
        <rdfs:label xml:lang="en">Event Identifier</rdfs:label>
    </owl:Class>
    


    <!-- https://w3id.org/cerif2/Event_Series -->


    <owl:Class rdf:about="https://w3id.org/cerif2/Event_Series">
        <rdfs:comment xml:lang="en">A thing that happens regularly (annually, bi-annually, etc.) about a particular subject.</rdfs:comment>
        <rdfs:label xml:lang="en">Event_Series</rdfs:label>
    </owl:Class>
    


    <!-- https://w3id.org/cerif2/Expertise_and_Skills -->


    <owl:Class rdf:about="https://w3id.org/cerif2/Expertise_and_Skills">
        <rdfs:comment xml:lang="en">**Expertise**: A high level of knowledge or skill.&lt;sup&gt;[1](#fn1)&lt;/sup&gt;

**Skill**: An ability to do an activity or job well, especially because you have practised it.&lt;sup&gt;[2](#fn2)&lt;/sup&gt;</rdfs:comment>
        <rdfs:label xml:lang="en">Expertise And Skills</rdfs:label>
    </owl:Class>
    


    <!-- https://w3id.org/cerif2/Expertise_and_Skills_Condition -->


    <owl:Class rdf:about="https://w3id.org/cerif2/Expertise_and_Skills_Condition">
        <rdfs:subClassOf rdf:resource="https://w3id.org/cerif2/Condition"/>
        <rdfs:comment xml:lang="en">The scope of the entity and its meaning.&lt;sup&gt;[1](#fn1)&lt;/sup&gt;</rdfs:comment>
        <rdfs:label xml:lang="en">Expertise and Skills Condition</rdfs:label>
    </owl:Class>
    


    <!-- https://w3id.org/cerif2/Expertise_and_Skills_Possession -->


    <owl:Class rdf:about="https://w3id.org/cerif2/Expertise_and_Skills_Possession">
        <rdfs:comment xml:lang="en">The statement of Possession of an [Expertise or Skill](../entities/Expertise_and_Skills.md) 
by an [Agent](../entities/Agent.md).</rdfs:comment>
        <rdfs:label xml:lang="en">Expertise and Skills Possession</rdfs:label>
    </owl:Class>
    


    <!-- https://w3id.org/cerif2/Expertise_and_Time_and_Effort -->


    <owl:Class rdf:about="https://w3id.org/cerif2/Expertise_and_Time_and_Effort">
        <rdfs:subClassOf rdf:resource="https://w3id.org/cerif2/Resource"/>
        <rdfs:comment xml:lang="en">**Expertise**: A high level of knowledge or skill.&lt;sup&gt;[1](#fn1)&lt;/sup&gt;

**Time**: An amount of time that you have available to do something.&lt;sup&gt;[2](#fn2)&lt;/sup&gt;

**Effort**: Physical or mental activity needed to achieve something.&lt;sup&gt;[3](#fn3)&lt;/sup&gt;</rdfs:comment>
        <rdfs:label xml:lang="en">Expertise and Time and Effort</rdfs:label>
    </owl:Class>
    


    <!-- https://w3id.org/cerif2/FundRef_Identifier -->


    <owl:Class rdf:about="https://w3id.org/cerif2/FundRef_Identifier">
        <rdfs:subClassOf rdf:resource="https://w3id.org/cerif2/Agent_Identifier"/>
        <rdfs:comment xml:lang="en">A FundRef&lt;sup&gt;[1](#fn1)&lt;/sup&gt; identifier assigned to an [Organisation unit](../entities/Organisation_Unit.md).</rdfs:comment>
        <rdfs:label xml:lang="en">FundRef Identifier</rdfs:label>
    </owl:Class>
    


    <!-- https://w3id.org/cerif2/Funding -->


    <owl:Class rdf:about="https://w3id.org/cerif2/Funding">
        <rdfs:subClassOf rdf:resource="https://w3id.org/cerif2/Resource"/>
        <rdfs:comment xml:lang="en">Money provided by an organization or government for a particular purpose.&lt;sup&gt;[1](#fn1)&lt;/sup&gt;</rdfs:comment>
        <rdfs:label xml:lang="en">Funding</rdfs:label>
    </owl:Class>
    


    <!-- https://w3id.org/cerif2/Funding_Application -->


    <owl:Class rdf:about="https://w3id.org/cerif2/Funding_Application">
        <rdfs:subClassOf rdf:resource="https://w3id.org/cerif2/Application"/>
        <rdfs:comment xml:lang="en">An application submitted in the form and manner described by a Funding agency, the purpose of which is to provide information to a Commission for project selection.&lt;sup&gt;[1](#fn1)&lt;/sup&gt;</rdfs:comment>
        <rdfs:label xml:lang="en">Funding Application</rdfs:label>
    </owl:Class>
    


    <!-- https://w3id.org/cerif2/Group -->


    <owl:Class rdf:about="https://w3id.org/cerif2/Group">
        <rdfs:subClassOf rdf:resource="https://w3id.org/cerif2/Group_or_Organisation_Unit"/>
        <rdfs:comment xml:lang="en">A non-formal group of [Agents](../entities/Agent.md).</rdfs:comment>
        <rdfs:label xml:lang="en">Group</rdfs:label>
    </owl:Class>
    


    <!-- https://w3id.org/cerif2/Group_or_Organisation_Unit -->


    <owl:Class rdf:about="https://w3id.org/cerif2/Group_or_Organisation_Unit">
        <rdfs:subClassOf rdf:resource="https://w3id.org/cerif2/Agent"/>
        <rdfs:comment xml:lang="en">A common supertype for [Group](../entities/Group.md) and [Organisation Unit](../entities/Organisation_Unit.md).</rdfs:comment>
        <rdfs:label xml:lang="en">Group or Organisation Unit</rdfs:label>
    </owl:Class>
    


    <!-- https://w3id.org/cerif2/ISNI_Identifier -->


    <owl:Class rdf:about="https://w3id.org/cerif2/ISNI_Identifier">
        <rdfs:subClassOf rdf:resource="https://w3id.org/cerif2/Agent_Identifier"/>
        <rdfs:comment xml:lang="en">An ISNI&lt;sup&gt;[1](#fn1)&lt;/sup&gt; identifier assigned to an [Agent](../entities/Agent.md).</rdfs:comment>
        <rdfs:label xml:lang="en">ISNI Identifier</rdfs:label>
    </owl:Class>
    


    <!-- https://w3id.org/cerif2/Infrastructure -->


    <owl:Class rdf:about="https://w3id.org/cerif2/Infrastructure">
        <rdfs:subClassOf rdf:resource="https://w3id.org/cerif2/Resource"/>
        <rdfs:comment xml:lang="en">The basic structure of an organization or system which is necessary for its operation, esp. public water, energy, and systems for communication and transport.&lt;sup&gt;[1](#fn1)&lt;/sup&gt;</rdfs:comment>
        <rdfs:label xml:lang="en">Infrastructure</rdfs:label>
    </owl:Class>
    


    <!-- https://w3id.org/cerif2/Involvement -->


    <owl:Class rdf:about="https://w3id.org/cerif2/Involvement">
        <rdfs:subClassOf rdf:resource="https://w3id.org/cerif2/Activity"/>
        <rdfs:comment xml:lang="en">The act or process of taking part in something,&lt;sup&gt;[1](#fn1)&lt;/sup&gt; namely in a [Group or Organisation Unit](../entities/Group_or_Organisation_Unit.md).</rdfs:comment>
        <rdfs:label xml:lang="en">Involvement</rdfs:label>
    </owl:Class>
    


    <!-- https://w3id.org/cerif2/Language -->


    <owl:Class rdf:about="https://w3id.org/cerif2/Language">
        <rdfs:comment xml:lang="en">A system of communication used by people living in a particular country consisting of sounds, words, and grammar.&lt;sup&gt;[1](#fn1)&lt;/sup&gt;</rdfs:comment>
        <rdfs:label xml:lang="en">Language</rdfs:label>
    </owl:Class>
    


    <!-- https://w3id.org/cerif2/Local_Agent_Identifier -->


    <owl:Class rdf:about="https://w3id.org/cerif2/Local_Agent_Identifier">
        <rdfs:subClassOf rdf:resource="https://w3id.org/cerif2/Agent_Identifier"/>
        <rdfs:comment xml:lang="en">A local identifier assigned to an [Agent](../entities/Agent.md). Local identifier is not adopted at global level, it 
might be some platform identifier, regional identifier or national identifier.</rdfs:comment>
        <rdfs:label xml:lang="en">Local Agent Identifier</rdfs:label>
    </owl:Class>
    


    <!-- https://w3id.org/cerif2/Local_Resource_Identifier -->


    <owl:Class rdf:about="https://w3id.org/cerif2/Local_Resource_Identifier">
        <rdfs:subClassOf rdf:resource="https://w3id.org/cerif2/Resource_Identifier"/>
        <rdfs:comment xml:lang="en">A local identifier assigned to a [Resource](../entities/Resource.md). Local identifier is not adopted at global level, it 
might be some platform identifier, regional identifier or national identifier.</rdfs:comment>
        <rdfs:label xml:lang="en">Local Resource Identifier</rdfs:label>
    </owl:Class>
    


    <!-- https://w3id.org/cerif2/Membership -->


    <owl:Class rdf:about="https://w3id.org/cerif2/Membership">
        <rdfs:subClassOf rdf:resource="https://w3id.org/cerif2/Involvement"/>
        <rdfs:comment xml:lang="en">The [Involvement](../entities/Involvement.md) of being a member in a [Group](../entities/Group.md).</rdfs:comment>
        <rdfs:label xml:lang="en">Membership</rdfs:label>
    </owl:Class>
    


    <!-- https://w3id.org/cerif2/Monetary_Amount -->


    <owl:Class rdf:about="https://w3id.org/cerif2/Monetary_Amount">
        <rdfs:comment xml:lang="en">A certain volume of money, together with the specification of a currency.</rdfs:comment>
        <rdfs:label xml:lang="en">Monetary Amount</rdfs:label>
    </owl:Class>
    


    <!-- https://w3id.org/cerif2/ORCID_Identifier -->


    <owl:Class rdf:about="https://w3id.org/cerif2/ORCID_Identifier">
        <rdfs:subClassOf rdf:resource="https://w3id.org/cerif2/Agent_Identifier"/>
        <rdfs:comment xml:lang="en">An ORCID&lt;sup&gt;[1](#fn1)&lt;/sup&gt; identifier assigned to a [Person](../entities/Person.md).</rdfs:comment>
        <rdfs:label xml:lang="en">ORCID Identifier</rdfs:label>
    </owl:Class>
    


    <!-- https://w3id.org/cerif2/Organisation_Unit -->


    <owl:Class rdf:about="https://w3id.org/cerif2/Organisation_Unit">
        <rdfs:subClassOf rdf:resource="https://w3id.org/cerif2/Group_or_Organisation_Unit"/>
        <rdfs:comment xml:lang="en">An Organisation or a part of an Organisation&apos;s structure.

**Organisation**: A formal, goal-orientated group with members and a defined structure, governed by rules and procedures that guide operation.&lt;sup&gt;[1](#fn1)&lt;/sup&gt;</rdfs:comment>
        <rdfs:label xml:lang="en">Organisation Unit</rdfs:label>
    </owl:Class>
    


    <!-- https://w3id.org/cerif2/Page_Based_Contents_Location -->


    <owl:Class rdf:about="https://w3id.org/cerif2/Page_Based_Contents_Location">
        <rdfs:subClassOf rdf:resource="https://w3id.org/cerif2/Contents_Location"/>
        <rdfs:comment xml:lang="en">A [Contents Location](../datatypes/Contents_Location.md) that is based on a range of pages.</rdfs:comment>
        <rdfs:label xml:lang="en">Page Based Contents Location</rdfs:label>
    </owl:Class>
    


    <!-- https://w3id.org/cerif2/Person -->


    <owl:Class rdf:about="https://w3id.org/cerif2/Person">
        <rdfs:subClassOf rdf:resource="https://w3id.org/cerif2/Agent"/>
        <rdfs:comment xml:lang="en">A human being as an individual.&lt;sup&gt;[1](#fn1)&lt;/sup&gt;</rdfs:comment>
        <rdfs:label xml:lang="en">Person</rdfs:label>
    </owl:Class>
    


    <!-- https://w3id.org/cerif2/Person_Name -->


    <owl:Class rdf:about="https://w3id.org/cerif2/Person_Name">
        <rdfs:comment xml:lang="en">The name of a [Person](../entities/Person.md).</rdfs:comment>
        <rdfs:label xml:lang="en">Person Name</rdfs:label>
    </owl:Class>
    


    <!-- https://w3id.org/cerif2/Physical_Address -->


    <owl:Class rdf:about="https://w3id.org/cerif2/Physical_Address">
        <rdfs:comment xml:lang="en">The location assigned to an [Organisation Unit](../entities/Organisation_Unit.md) or some other CERIF entity instance.</rdfs:comment>
        <rdfs:label xml:lang="en">Physical Address</rdfs:label>
    </owl:Class>
    


    <!-- https://w3id.org/cerif2/Position -->


    <owl:Class rdf:about="https://w3id.org/cerif2/Position">
        <rdfs:comment xml:lang="en">A rank or level in a company, competition, or society.&lt;sup&gt;[1](#fn1)&lt;/sup&gt;</rdfs:comment>
        <rdfs:label xml:lang="en">Position</rdfs:label>
    </owl:Class>
    


    <!-- https://w3id.org/cerif2/Postal_Address -->


    <owl:Class rdf:about="https://w3id.org/cerif2/Postal_Address">
        <rdfs:subClassOf rdf:resource="https://w3id.org/cerif2/Contact_Information"/>
        <rdfs:comment xml:lang="en">A postal address assigned to an [Agent](../entities/Organisation_Unit.md).</rdfs:comment>
        <rdfs:label xml:lang="en">Postal Address</rdfs:label>
    </owl:Class>
    


    <!-- https://w3id.org/cerif2/Prize -->


    <owl:Class rdf:about="https://w3id.org/cerif2/Prize">
        <rdfs:comment xml:lang="en">Something valuable, such as an amount of money, that is given to someone who succeeds in a competition or game or that is given to someone as a reward for doing very good work.&lt;sup&gt;[1](#fn1)&lt;/sup&gt;</rdfs:comment>
        <rdfs:label xml:lang="en">Prize</rdfs:label>
    </owl:Class>
    


    <!-- https://w3id.org/cerif2/Prize_Award -->


    <owl:Class rdf:about="https://w3id.org/cerif2/Prize_Award">
        <rdfs:comment xml:lang="en">A [prize](../entities/Prize.md) or a sum of money that a person or organization is given for an achievement.&lt;sup&gt;[1](#fn1)&lt;/sup&gt;</rdfs:comment>
        <rdfs:label xml:lang="en">Prize Award</rdfs:label>
    </owl:Class>
    


    <!-- https://w3id.org/cerif2/Project -->


    <owl:Class rdf:about="https://w3id.org/cerif2/Project">
        <rdfs:comment xml:lang="en">A temporary endeavor undertaken to create a unique product, service or result.&lt;br/&gt;
Source: the Project Management Institute, https://www.pmi.org/about/learn-about-pmi/what-is-project-management</rdfs:comment>
        <rdfs:label xml:lang="en">Project</rdfs:label>
    </owl:Class>
    


    <!-- https://w3id.org/cerif2/Publication_Channel -->


    <owl:Class rdf:about="https://w3id.org/cerif2/Publication_Channel">
        <rdfs:comment xml:lang="en">A Publication Channel is a medium for publishing documents.</rdfs:comment>
        <rdfs:label xml:lang="en">Publication Channel</rdfs:label>
    </owl:Class>
    


    <!-- https://w3id.org/cerif2/ROR_Identifier -->


    <owl:Class rdf:about="https://w3id.org/cerif2/ROR_Identifier">
        <rdfs:subClassOf rdf:resource="https://w3id.org/cerif2/Agent_Identifier"/>
        <rdfs:comment xml:lang="en">A ROR&lt;sup&gt;[1](#fn1)&lt;/sup&gt; identifier assigned to an [Organisation unit](../entities/Organisation_Unit.md).</rdfs:comment>
        <rdfs:label xml:lang="en">ROR Identifier</rdfs:label>
    </owl:Class>
    


    <!-- https://w3id.org/cerif2/Repository -->


    <owl:Class rdf:about="https://w3id.org/cerif2/Repository">
        <rdfs:subClassOf rdf:resource="https://w3id.org/cerif2/Infrastructure"/>
        <rdfs:subClassOf rdf:resource="https://w3id.org/cerif2/Publication_Channel"/>
        <rdfs:comment xml:lang="en">A place where things are stored and can be found.&lt;sup&gt;[1](#fn1)&lt;/sup&gt;</rdfs:comment>
        <rdfs:label xml:lang="en">Repository</rdfs:label>
    </owl:Class>
    


    <!-- https://w3id.org/cerif2/Resource -->


    <owl:Class rdf:about="https://w3id.org/cerif2/Resource">
        <rdfs:comment xml:lang="en">Anything that can be used for or in the process of research.</rdfs:comment>
        <rdfs:label xml:lang="en">Resource</rdfs:label>
    </owl:Class>
    


    <!-- https://w3id.org/cerif2/Resource_Identifier -->


    <owl:Class rdf:about="https://w3id.org/cerif2/Resource_Identifier">
        <rdfs:comment xml:lang="en">An identifier that is assigned to a [Resource](../entities/Resource.md).</rdfs:comment>
        <rdfs:label xml:lang="en">Resource Identifier</rdfs:label>
    </owl:Class>
    


    <!-- https://w3id.org/cerif2/Resource_Offer -->


    <owl:Class rdf:about="https://w3id.org/cerif2/Resource_Offer">
        <rdfs:comment xml:lang="en">An offer of a [Resource](../entities/Resource.md) for usage.</rdfs:comment>
        <rdfs:label xml:lang="en">Resource Offer</rdfs:label>
    </owl:Class>
    


    <!-- https://w3id.org/cerif2/Resource_Request -->


    <owl:Class rdf:about="https://w3id.org/cerif2/Resource_Request">
        <rdfs:comment xml:lang="en">A request to use a [Resource](../entities/Resource.md).</rdfs:comment>
        <rdfs:label xml:lang="en">Resource Request</rdfs:label>
    </owl:Class>
    


    <!-- https://w3id.org/cerif2/Resource_Usage_Statement -->


    <owl:Class rdf:about="https://w3id.org/cerif2/Resource_Usage_Statement">
        <rdfs:comment xml:lang="en">An element of a [Contribution](../entities/Contribution.md). All such elements taken together describe the Contribution.</rdfs:comment>
        <rdfs:label xml:lang="en">Resource Usage Statement</rdfs:label>
    </owl:Class>
    


    <!-- https://w3id.org/cerif2/Script -->


    <owl:Class rdf:about="https://w3id.org/cerif2/Script">
        <rdfs:comment xml:lang="en">Script indicates writing system variations that distinguish the written forms of a language or its dialects&lt;sup&gt;[1](#fn1)&lt;/sup&gt;</rdfs:comment>
        <rdfs:label xml:lang="en">Script</rdfs:label>
    </owl:Class>
    


    <!-- https://w3id.org/cerif2/Simple_Physical_Address -->


    <owl:Class rdf:about="https://w3id.org/cerif2/Simple_Physical_Address">
        <rdfs:subClassOf rdf:resource="https://w3id.org/cerif2/Physical_Address"/>
        <rdfs:comment xml:lang="en">This data type is used when a string representation of physical address is used.</rdfs:comment>
        <rdfs:label xml:lang="en">Simple Postal Address</rdfs:label>
    </owl:Class>
    


    <!-- https://w3id.org/cerif2/Structured_Physical_Address -->


    <owl:Class rdf:about="https://w3id.org/cerif2/Structured_Physical_Address">
        <rdfs:subClassOf rdf:resource="https://w3id.org/cerif2/Physical_Address"/>
        <rdfs:comment xml:lang="en">This data type is used when a structured representation of physical address is used.</rdfs:comment>
        <rdfs:label xml:lang="en">Structured Postal Address</rdfs:label>
    </owl:Class>
    


    <!-- https://w3id.org/cerif2/Tangible -->


    <owl:Class rdf:about="https://w3id.org/cerif2/Tangible">
        <rdfs:comment xml:lang="en">Something that is real and able to be shown or touched.&lt;sup&gt;[1](#fn1)&lt;/sup&gt;</rdfs:comment>
        <rdfs:label xml:lang="en">Tangible</rdfs:label>
    </owl:Class>
    


    <!-- https://w3id.org/cerif2/Textual_Contents -->


    <owl:Class rdf:about="https://w3id.org/cerif2/Textual_Contents">
        <rdfs:comment xml:lang="en">A resource consisting primarily of words for reading.&lt;sup&gt;[1](#fn1)&lt;/sup&gt;</rdfs:comment>
        <rdfs:label xml:lang="en">Textual Contents</rdfs:label>
    </owl:Class>
    


    <!-- https://w3id.org/cerif2/Time_Based_Contents_Location -->


    <owl:Class rdf:about="https://w3id.org/cerif2/Time_Based_Contents_Location">
        <rdfs:subClassOf rdf:resource="https://w3id.org/cerif2/Contents_Location"/>
        <rdfs:comment xml:lang="en">A [Contents Location](../datatypes/Contents_Location.md) that is based on a time interval.</rdfs:comment>
        <rdfs:label xml:lang="en">Time Based Contents Location</rdfs:label>
    </owl:Class>
    


    <!-- https://w3id.org/cerif2/Video_Contents -->


    <owl:Class rdf:about="https://w3id.org/cerif2/Video_Contents">
        <rdfs:comment xml:lang="en">Media that makes use of images (usually &quot;moving&quot;), with or without sound, over a period of playback time.&lt;sup&gt;[1](#fn1)&lt;/sup&gt;</rdfs:comment>
        <rdfs:label xml:lang="en">Video Contents</rdfs:label>
    </owl:Class>
    


    <!-- https://w3id.org/cerif2/Visiting_Address -->


    <owl:Class rdf:about="https://w3id.org/cerif2/Visiting_Address">
        <rdfs:subClassOf rdf:resource="https://w3id.org/cerif2/Contact_Information"/>
        <rdfs:comment xml:lang="en">A visiting address assigned to an [Agent](../entities/Organisation_Unit.md).</rdfs:comment>
        <rdfs:label xml:lang="en">Visiting Address</rdfs:label>
    </owl:Class>
    


    <!-- https://w3id.org/cerif2/Wikidata_Agent_Identifier -->


    <owl:Class rdf:about="https://w3id.org/cerif2/Wikidata_Agent_Identifier">
        <rdfs:subClassOf rdf:resource="https://w3id.org/cerif2/Agent_Identifier"/>
        <rdfs:comment xml:lang="en">A Wikidata&lt;sup&gt;[1](#fn1)&lt;/sup&gt; identifier assigned to an [Agent](../entities/Agent.md).</rdfs:comment>
        <rdfs:label xml:lang="en">Wikidata Agent Identifier</rdfs:label>
    </owl:Class>
    


    <!-- https://w3id.org/cerif2/Wikidata_Resource_Identifier -->


    <owl:Class rdf:about="https://w3id.org/cerif2/Wikidata_Resource_Identifier">
        <rdfs:subClassOf rdf:resource="https://w3id.org/cerif2/Resource_Identifier"/>
        <rdfs:comment xml:lang="en">A Wikidata&lt;sup&gt;[1](#fn1)&lt;/sup&gt; identifier assigned to a [Resource](../entities/Resource.md).</rdfs:comment>
        <rdfs:label xml:lang="en">Wikidata Resource Identifier</rdfs:label>
    </owl:Class>
</rdf:RDF>



<!-- Generated by the OWL API (version 5.5.1) https://github.com/owlcs/owlapi/ -->


